refactoring

crypto/ec/Hacl.EC.Curve25519.Bignum.Fdifference.fst
@@ -12,7 +12,6 @@ open Hacl.UInt64
 open Hacl.EC.Curve25519.Parameters
 open Hacl.EC.Curve25519.Bigint
 open Hacl.EC.Curve25519.Utils
-open Hacl.EC.Curve25519.Bignum.Fdifference.Lemmas
 
 #reset-options "--initial_fuel 0 --max_fuel 0"
 
@@ -31,48 +30,39 @@ module H64  = Hacl.UInt64
 val add_big_zero_:
   b:bigint ->
   Stack unit
-    (requires (fun h -> norm h b))
-    (ensures (fun h0 _ h1 -> addedZero h0 h1 b /\ modifies_1 b h0 h1))
+    (requires (fun h -> live h b))
+    (ensures (fun h0 _ h1 -> live h1 b /\ modifies_1 b h0 h1))
 let add_big_zero_ b =
   let two52m38 = (Hacl.Cast.uint64_to_sint64 0xfffffffffffdauL) in // pow2 52 - 38
   let two52m2 =  (Hacl.Cast.uint64_to_sint64 0xffffffffffffeuL) in // pow2 52 - 2
-  lemma_pow2_52m38 ();
-  lemma_pow2_52m2 ();
-  cut(v two52m38 = pow2 52 - 38 /\ v two52m2 = pow2 52 - 2);
   let b0 = b.(0ul) in
   let b1 = b.(1ul) in
   let b2 = b.(2ul) in
   let b3 = b.(3ul) in
   let b4 = b.(4ul) in
-  lemma_add_big_zero_core b0 b1 b2 b3 b4;
-  let c0 = b0 +^ two52m38 in
-  let c1 = b1 +^ two52m2  in
-  let c2 = b2 +^ two52m2  in
-  let c3 = b3 +^ two52m2  in
-  let c4 = b4 +^ two52m2  in
+  let c0 = b0 +%^ two52m38 in
+  let c1 = b1 +%^ two52m2  in
+  let c2 = b2 +%^ two52m2  in
+  let c3 = b3 +%^ two52m2  in
+  let c4 = b4 +%^ two52m2  in
   update_5 b c0 c1 c2 c3 c4
 
 
 val add_big_zero:
   b:bigint ->
   Stack unit
-    (requires (fun h -> norm h b))
-    (ensures (fun h0 _ h1 -> live h0 b /\ fits51to53 h1 b /\ modifies_1 b h0 h1
-      /\ eval h1 b norm_length % reveal prime = eval h0 b norm_length % reveal prime))
+    (requires (fun h -> live h b))
+    (ensures (fun h0 _ h1 -> live h1 b /\ modifies_1 b h0 h1))
 let add_big_zero b =
-  let h0 = ST.get() in
-  add_big_zero_ b;
-  let h1 = ST.get() in
-  lemma_add_zero_eval h0 h1 b
+  add_big_zero_ b
 
 
 val fdifference_:
   a:bigint ->
   b:bigint{disjoint a b} ->
   Stack unit
-    (requires (fun h -> norm h a /\ fits51to53 h b))
-    (ensures (fun h0 _ h1 -> bound53 h1 a /\ modifies_1 a h0 h1
-      /\ isDifference h0 h1 a b))
+    (requires (fun h -> live h a /\ live h b))
+    (ensures (fun h0 _ h1 -> live h1 a /\ modifies_1 a h0 h1))
 let fdifference_ a b =
   let a0 = a.(0ul) in
   let a1 = a.(1ul) in
@@ -84,11 +74,11 @@ let fdifference_ a b =
   let b2 = b.(2ul) in
   let b3 = b.(3ul) in
   let b4 = b.(4ul) in
-  let c0 = b0 -^ a0 in
-  let c1 = b1 -^ a1 in
-  let c2 = b2 -^ a2 in
-  let c3 = b3 -^ a3 in
-  let c4 = b4 -^ a4 in
+  let c0 = b0 -%^ a0 in
+  let c1 = b1 -%^ a1 in
+  let c2 = b2 -%^ a2 in
+  let c3 = b3 -%^ a3 in
+  let c4 = b4 -%^ a4 in
   update_5 a c0 c1 c2 c3 c4
 
 
@@ -96,12 +86,7 @@ val fdifference':
   a:bigint ->
   b:bigint{disjoint a b} ->
   Stack unit
-    (requires (fun h -> norm h a /\ fits51to53 h b))
-    (ensures (fun h0 u h1 -> live h0 a /\ live h0 b /\ bound53 h1 a /\ modifies_1 a h0 h1
-      /\ eval h1 a norm_length
-        = eval h0 b norm_length - eval h0 a norm_length))
+    (requires (fun h -> live h a /\ live h b))
+    (ensures (fun h0 u h1 -> live h1 a /\ modifies_1 a h0 h1))
 let fdifference' a b =
-  let h0 = ST.get() in
-  fdifference_ a b;
-  let h1 = ST.get() in
-  lemma_fdifference h0 h1 a b
+  fdifference_ a b
