crypto/ec/Hacl.EC.Curve25519.Bignum.Modulo.fst
@@ -14,8 +14,6 @@ open Hacl.EC.Curve25519.Parameters
 open Hacl.EC.Curve25519.Bigint
 open Hacl.EC.Curve25519.Utils
 
-open Hacl.EC.Curve25519.Bignum.Modulo.Lemmas
-
 #reset-options "--initial_fuel 0 --max_fuel 0"
 
 (* Module abbreviations *)
@@ -32,26 +30,21 @@ module H128  = Hacl.UInt128
 
 #reset-options "--initial_fuel 0 --max_fuel 0 --z3timeout 5"
 
-val times_wide_19: x:s128{19 * H128.v x < pow2 platform_wide} -> Tot (y:s128{H128.v y = 19 * H128.v x})
-let times_wide_19 x =
+inline_for_extraction val times_wide_19: s128 -> Tot (s128)
+inline_for_extraction let times_wide_19 x =
   let open Hacl.UInt128 in
-  assert_norm (pow2 128 = 340282366920938463463374607431768211456);
-  assert_norm (pow2 4 = 16);
-  assert_norm (pow2 1 = 2);
   let y = x <<^ 4ul in
-  modulo_lemma (pow2 4 * v x) (pow2 128);
   let z = x <<^ 1ul in
-  modulo_lemma (pow2 1 * v x) (pow2 128);
-  x +^ y +^ z
+  x +%^ y +%^ z
 
 
 #reset-options "--initial_fuel 0 --max_fuel 0 --z3timeout 20"
 
 val freduce_degree_:
-  b:bigint_wide ->
+  b:bigint_wide{length b >= 2*norm_length-1} ->
   Stack unit
-    (requires (fun h -> satisfiesModuloConstraints h b))
-    (ensures (fun h0 _ h1 -> isDegreeReduced h0 h1 b /\ modifies_1 b h0 h1))
+    (requires (fun h -> live h b))
+    (ensures (fun h0 _ h1 -> live h1 b /\ modifies_1 b h0 h1))
 let freduce_degree_ b =
   let h0 = ST.get() in
   let b0 = b.(0ul) in
@@ -62,12 +55,11 @@ let freduce_degree_ b =
   let b6 = b.(6ul) in
   let b7 = b.(7ul) in
   let b8 = b.(8ul) in
-  lemma_freduce_degree_0 h0 b;
   let open Hacl.UInt128 in
-  let b0' = b0 +^ times_wide_19 b5 in
-  let b1' = b1 +^ times_wide_19 b6 in
-  let b2' = b2 +^ times_wide_19 b7 in
-  let b3' = b3 +^ times_wide_19 b8 in
+  let b0' = b0 +%^ times_wide_19 b5 in
+  let b1' = b1 +%^ times_wide_19 b6 in
+  let b2' = b2 +%^ times_wide_19 b7 in
+  let b3' = b3 +%^ times_wide_19 b8 in
   b.(0ul) <- b0';
   b.(1ul) <- b1';
   b.(2ul) <- b2';
@@ -75,83 +67,45 @@ let freduce_degree_ b =
 
 
 val freduce_degree:
-  b:bigint_wide ->
+  b:bigint_wide{length b >= 2*norm_length - 1} ->
   Stack unit
-    (requires (fun h -> satisfiesModuloConstraints h b))
-    (ensures (fun h0 _ h1 -> modifies_1 b h0 h1
-      /\ satisfiesModuloConstraints h0 b
-      /\ bound127 h1 b
-      /\ eval_wide h1 b norm_length % reveal prime = eval_wide h0 b (2*norm_length-1) % reveal prime))
+    (requires (fun h -> live h b))
+    (ensures (fun h0 _ h1 -> modifies_1 b h0 h1 /\ live h1 b))
 let freduce_degree b =
-  let h0 = ST.get() in
-  freduce_degree_ b;
-  let h1 = ST.get() in
-  lemma_freduce_degree h0 h1 b
+  freduce_degree_ b
 
-val mod_wide_2_51: a:s128 -> Tot (b:s128{H128.v b = H128.v a % pow2 51})
-let mod_wide_2_51 a =
-  let open Hacl.UInt128 in
+inline_for_extraction val mod_wide_2_51: a:s128 -> Tot s128
+inline_for_extraction let mod_wide_2_51 a =
   let mask = (Hacl.Cast.uint64_to_sint128 0x7ffffffffffffuL) in
-  assert_norm(v mask = pow2 51 - 1);
-  let res = a &^ mask in
-  UInt.logand_mask #128 (v a) 51;
-  res
+  H128 (a &^ mask)
 
 
-private val div_wide_2_51: x:s128 -> Tot (y:s128{H128.v y = H128.v x / pow2 51 /\ H128.v y <= pow2 77})
-let div_wide_2_51 x = 
+inline_for_extraction private val div_wide_2_51: x:s128 -> Tot (s128)
+inline_for_extraction private let div_wide_2_51 x = 
   let open Hacl.UInt128 in
-  pow2_minus 128 51; lemma_div_mod (H128.v x) (pow2 51);
-  lemma_div_lt (v x) 128 51;
   (x >>^ 51ul)
-
-
-let isCarriedWide_
-  (h1:mem)
-  (b0:H128.t) (b1:H128.t) (b2:H128.t) (b3:H128.t) (b4:H128.t)
-  (b:bigint_wide) : GTot Type0 =
-  live h1 b /\ length b >= norm_length+1
-  /\ (
-      let open Hacl.UInt128 in
-      let r0  = v b0 / pow2 51 in
-      let r1  = (v b1 + r0) / pow2 51 in
-      let r2  = (v b2 + r1) / pow2 51 in
-      let r3  = (v b3 + r2) / pow2 51 in
-      v (get h1 b 5) = (v b4 + r3) / pow2 51
-      /\ v (get h1 b 0) = v b0 % pow2 51
-      /\ v (get h1 b 1) = (v b1 + r0)  % pow2 51
-      /\ v (get h1 b 2) = (v b2 + r1)  % pow2 51
-      /\ v (get h1 b 3) = (v b3 + r2)  % pow2 51
-      /\ v (get h1 b 4) = (v b4 + r3)  % pow2 51
-    )
 
 
 #reset-options "--initial_fuel 0 --max_fuel 0 --z3timeout 20"
 
 private val carry_wide_1_0:
   b:bigint_wide{length b >= norm_length+1} ->
-  b0:u127 -> b1:u127 -> b2:u127 -> b3:u127 -> b4:u127 ->
+  b0:H128.t -> b1:H128.t -> b2:H128.t -> b3:H128.t -> b4:H128.t ->
   Stack unit
-    (requires (fun h -> bound127 h b))
-    (ensures (fun h0 _ h1 -> bound127 h0 b /\ norm_wide h1 b /\ modifies_1 b h0 h1
-      /\ isCarriedWide_ h1 b0 b1 b2 b3 b4 b ))
+    (requires (fun h -> live h b))
+    (ensures (fun h0 _ h1 -> live h1 b /\ modifies_1 b h0 h1))
 let carry_wide_1_0 b b0 b1 b2 b3 b4 =
-  assert_norm (pow2 51 = 2251799813685248);
-  assert_norm (pow2 77 = 151115727451828646838272);
-  pow2_lt_compat 78 77; pow2_lt_compat 127 78; pow2_double_sum 127;
-  assert(forall x y. {:pattern (v x + v y)}(v x < pow2 127 /\ v y <= pow2 77)
-    ==> v x + v y < pow2 128);
   let b0' = mod_wide_2_51 b0 in
   let r0  = div_wide_2_51 b0 in
   let open Hacl.UInt128 in
-  let b1' = mod_wide_2_51 (b1 +^ r0) in
-  let r1  = div_wide_2_51 (b1 +^ r0) in
-  let b2' = mod_wide_2_51 (b2 +^ r1) in
-  let r2  = div_wide_2_51 (b2 +^ r1) in
-  let b3' = mod_wide_2_51 (b3 +^ r2) in
-  let r3  = div_wide_2_51 (b3 +^ r2) in
-  let b4' = mod_wide_2_51 (b4 +^ r3) in
-  let b5' = div_wide_2_51 (b4 +^ r3) in
+  let b1' = mod_wide_2_51 (b1 +%^ r0) in
+  let r1  = div_wide_2_51 (b1 +%^ r0) in
+  let b2' = mod_wide_2_51 (b2 +%^ r1) in
+  let r2  = div_wide_2_51 (b2 +%^ r1) in
+  let b3' = mod_wide_2_51 (b3 +%^ r2) in
+  let r3  = div_wide_2_51 (b3 +%^ r2) in
+  let b4' = mod_wide_2_51 (b4 +%^ r3) in
+  let b5' = div_wide_2_51 (b4 +%^ r3) in
   update_wide_6 b b0' b1' b2' b3' b4' b5'
 
 
@@ -160,9 +114,8 @@ let carry_wide_1_0 b b0 b1 b2 b3 b4 =
 private val carry_wide_1_:
   b:bigint_wide{length b >= norm_length+1} ->
   Stack unit
-    (requires (fun h -> bound127 h b))
-    (ensures (fun h0 _ h1 -> bound127 h0 b /\ norm_wide h1 b /\ modifies_1 b h0 h1
-      /\ isCarried h0 h1 b))
+    (requires (fun h -> live h b))
+    (ensures (fun h0 _ h1 -> live h1 b /\ modifies_1 b h0 h1))
 let carry_wide_1_ b =
   let b0 = b.(0ul) in
   let b1 = b.(1ul) in
@@ -175,123 +128,86 @@ let carry_wide_1_ b =
 val carry_wide_1:
   b:bigint_wide{length b >= norm_length+1} ->
   Stack unit
-    (requires (fun h -> bound127 h b))
-    (ensures (fun h0 _ h1 -> bound127 h0 b /\ norm_wide h1 b /\ modifies_1 b h0 h1
-      /\ eval_wide h1 b (norm_length+1) = eval_wide h0 b norm_length /\ carried_1 h1 b))
+    (requires (fun h -> live h b))
+    (ensures (fun h0 _ h1 -> live h1 b /\ modifies_1 b h0 h1))
 let carry_wide_1 b =
-  let h0 = ST.get() in
-  carry_wide_1_ b;
-  let h1 = ST.get() in
-  lemma_carry_1 h0 h1 b
+  carry_wide_1_ b
 
 
 val carry_wide_2_:
-  b:bigint_wide ->
+  b:bigint_wide{length b >= norm_length+1} ->
   Stack unit
-    (requires (fun h -> carried_2 h b))
-    (ensures (fun h0 _ h1 -> live h0 b /\ norm_wide h1 b /\ modifies_1 b h0 h1
-      /\ isCarried h0 h1 b))
+    (requires (fun h -> live h b))
+    (ensures (fun h0 _ h1 -> live h1 b /\ modifies_1 b h0 h1))
 let carry_wide_2_ b =
-  pow2_lt_compat 127 83; pow2_lt_compat 127 51;
   carry_wide_1_ b
 
 
 val carry_wide_2:
-  b:bigint_wide ->
+  b:bigint_wide{length b >= norm_length+1} ->
   Stack unit
-    (requires (fun h -> carried_2 h b))
-    (ensures (fun h0 _ h1 -> carried_2 h0 b /\ norm_wide h1 b /\ modifies_1 b h0 h1
-	  /\ eval_wide h1 b (norm_length+1) = eval_wide h0 b norm_length
-	  /\ carried_3 h1 b))
+    (requires (fun h -> live h b))
+    (ensures (fun h0 _ h1 -> live h1 b /\ modifies_1 b h0 h1))
 let carry_wide_2 b =
-  let h0 = ST.get() in
-  carry_wide_2_ b;
-  let h1 = ST.get() in
-  lemma_carry_2 h0 h1 b
-
+  carry_wide_2_ b
 
 val carry_wide_top_:
   b:bigint_wide ->
   Stack unit
-    (requires (fun h -> live h b /\ length b >= norm_length+1
-      /\ (let open Hacl.UInt128 in v (get h b 0) + 19 * v (get h b 5) < pow2 128 )))
-    (ensures  (fun h0 _ h1 -> live h1 b /\ modifies_1 b h0 h1
-      /\ carriedTopBottom h0 h1 b))
+    (requires (fun h -> live h b /\ length b >= norm_length+1))
+    (ensures  (fun h0 _ h1 -> live h1 b /\ modifies_1 b h0 h1))
 let carry_wide_top_ b =
   let b0 = b.(0ul) in
   let b5 = b.(5ul) in
-  b.(0ul) <- H128 (b0 +^ times_wide_19 b5)
+  b.(0ul) <- H128 (b0 +%^ times_wide_19 b5)
 
 
 val carry_wide_top_1:
-  b:bigint_wide ->
+  b:bigint_wide{length b >= norm_length+1} ->
   Stack unit
-    (requires (fun h -> carried_1 h b))
-    (ensures  (fun h0 _ h1 -> carried_1 h0 b /\ carried_2 h1 b /\ modifies_1 b h0 h1
-      /\ eval_wide h1 b norm_length % reveal prime = eval_wide h0 b (norm_length+1) % reveal prime))
+    (requires (fun h -> live h b))
+    (ensures  (fun h0 _ h1 -> live h1 b /\ modifies_1 b h0 h1))
 let carry_wide_top_1 b =
-  let h0 = ST.get() in
-  assert_norm (pow2 51 = 2251799813685248);
-  assert_norm (pow2 77 = 151115727451828646838272);
-  assert_norm (pow2 128 = 340282366920938463463374607431768211456);
-  carry_wide_top_ b;
-  let h1 = ST.get() in
-  lemma_carry_top_1 h0 h1 b
+  carry_wide_top_ b
 
 
 val carry_wide_top_2:
-  b:bigint_wide ->
+  b:bigint_wide{length b >= norm_length + 1} ->
   Stack unit
-    (requires (fun h -> carried_3 h b))
-    (ensures  (fun h0 _ h1 -> carried_3 h0 b /\ carried_4 h1 b /\ modifies_1 b h0 h1
-      /\ eval_wide h1 b norm_length % reveal prime = eval_wide h0 b (norm_length+1) % reveal prime))
+    (requires (fun h -> live h b))
+    (ensures  (fun h0 _ h1 -> live h1 b /\ modifies_1 b h0 h1))
 let carry_wide_top_2 b =
-  let h0 = ST.get() in
-  assert_norm (pow2 5 = 32);
-  assert_norm (pow2 51 = 2251799813685248);
-  assert_norm (pow2 77 = 151115727451828646838272);
-  assert_norm (pow2 128 = 340282366920938463463374607431768211456);
-  carry_wide_top_ b;
-  let h1 = ST.get() in
-  lemma_carry_top_2 h0 h1 b
+  carry_wide_top_ b
 
 
 private val carry_wide_0_to_1_:
-  b:bigint_wide ->
+  b:bigint_wide{length b >= norm_length + 1} ->
   Stack unit
-    (requires (fun h -> carried_4 h b))
-    (ensures  (fun h0 _ h1 -> isCarried01 h0 h1 b /\ modifies_1 b h0 h1))
+    (requires (fun h -> live h b))
+    (ensures  (fun h0 _ h1 -> live h1 b /\ modifies_1 b h0 h1))
 let carry_wide_0_to_1_ b =
-  assert_norm (pow2 51 = 2251799813685248);
-  assert_norm (pow2 77 = 151115727451828646838272);
-  assert_norm (pow2 128 = 340282366920938463463374607431768211456);
   let b0 = b.(0ul) in
   let b1 = b.(1ul) in
   let b0' = mod_wide_2_51 b0 in
   let r0  = div_wide_2_51 b0 in
   b.(0ul) <- b0';
-  b.(1ul) <- H128 (b1 +^ r0)
+  b.(1ul) <- H128 (b1 +%^ r0)
 
 
 val carry_wide_0_to_1:
-  b:bigint_wide ->
+  b:bigint_wide{length b >= norm_length + 1} ->
   Stack unit
-    (requires (fun h -> carried_4 h b))
-    (ensures  (fun h0 _ h1 -> carried_4 h0 b /\ modifies_1 b h0 h1 /\ norm_wide h1 b
-      /\ eval_wide h1 b norm_length = eval_wide h0 b norm_length))
+    (requires (fun h -> live h b))
+    (ensures  (fun h0 _ h1 -> modifies_1 b h0 h1 /\ live h1 b))
 let carry_wide_0_to_1 b =
-  let h0 = ST.get() in
-  carry_wide_0_to_1_ b;
-  let h1 = ST.get() in
-  lemma_carry_0_to_1 h0 h1 b
+  carry_wide_0_to_1_ b
 
 
 val freduce_coefficients_wide:
   b:bigint_wide{length b >= norm_length + 1} ->
   Stack unit
-    (requires (fun h -> bound127 h b))
-    (ensures (fun h0 _ h1 -> bound127 h0 b /\ norm_wide h1 b /\ modifies_1 b h0 h1
-      /\ eval_wide h1 b norm_length % reveal prime = eval_wide h0 b norm_length % reveal prime))
+    (requires (fun h -> live h b))
+    (ensures (fun h0 _ h1 -> live h1 b /\ modifies_1 b h0 h1))
 let freduce_coefficients_wide b =
   carry_wide_1 b;
   carry_wide_top_1 b;
@@ -302,109 +218,43 @@ let freduce_coefficients_wide b =
 
 (*******************************************************************************)
 
-open Hacl.EC.Curve25519.Bignum.Modulo.Lemmas2
-
-val times_19: x:s64{19 * v x < pow2 64} -> Tot (y:s64{v y = 19 * v x})
-let times_19 x =
-  assert_norm (pow2 64 = 18446744073709551616);
-  assert_norm (pow2 4 = 16);
-  assert_norm (pow2 1 = 2);
+inline_for_extraction val times_19: x:s64 -> Tot s64
+inline_for_extraction let times_19 x =
   let y = x <<^ 4ul in
-  modulo_lemma (pow2 4 * v x) (pow2 64);
   let z = x <<^ 1ul in
-  modulo_lemma (pow2 1 * v x) (pow2 64);
-  x +^ y +^ z
+  x +%^ y +%^ z
 
 
-
-val mod_2_51: a:s64 -> Tot (b:s64{H64.v b = H64.v a % pow2 51})
-let mod_2_51 a =
+inline_for_extraction val mod_2_51: a:s64 -> Tot s64
+inline_for_extraction let mod_2_51 a =
   let open Hacl.UInt64 in
   let mask = (Hacl.Cast.uint64_to_sint64 0x7ffffffffffffuL) in
-  assert_norm(v mask = pow2 51 - 1);
-  let res = a &^ mask in
-  UInt.logand_mask #64 (v a) 51;
-  res
+  a &^ mask
 
 
-private val div_2_51: x:s64 -> Tot (y:s64{H64.v y = H64.v x / pow2 51 /\ H64.v y <= pow2 13})
-let div_2_51 x =
+inline_for_extraction private val div_2_51: x:s64 -> Tot s64
+inline_for_extraction private let div_2_51 x =
   let open Hacl.UInt64 in
-  pow2_minus 64 51; lemma_div_mod (H64.v x) (pow2 51);
-  lemma_div_lt (v x) 64 51;
   (x >>^ 51ul)
 
 
-let isCarried_'
-  (h1:mem)
-  (b0:H64.t) (b1:H64.t) (b2:H64.t) (b3:H64.t) (b4:H64.t)
-  (b:bigint) : GTot Type0 =
-  live h1 b /\ length b >= norm_length+1
-  /\ (
-      let r0  = v b0 / pow2 51 in
-      let r1  = (v b1 + r0) / pow2 51 in
-      let r2  = (v b2 + r1) / pow2 51 in
-      let r3  = (v b3 + r2) / pow2 51 in
-      v (get h1 b 5) = (v b4 + r3) / pow2 51
-      /\ v (get h1 b 0) = v b0 % pow2 51
-      /\ v (get h1 b 1) = (v b1 + r0)  % pow2 51
-      /\ v (get h1 b 2) = (v b2 + r1)  % pow2 51
-      /\ v (get h1 b 3) = (v b3 + r2)  % pow2 51
-      /\ v (get h1 b 4) = (v b4 + r3)  % pow2 51
-    )
-
-(* let isCarried (h0:mem) (h1:mem) (b:bigint) : GTot Type0 = *)
-(*   live h0 b /\ live h1 b /\ length b >= norm_length+1 *)
-(*   /\ ( *)
-(*       let b0 = v (get h0 b 0) in *)
-(*       let b1 = v (get h0 b 1) in *)
-(*       let b2 = v (get h0 b 2) in *)
-(*       let b3 = v (get h0 b 3) in *)
-(*       let b4 = v (get h0 b 4) in *)
-(*       let r0  = b0 / pow2 51 in *)
-(*       let r1  = (b1 + r0) / pow2 51 in *)
-(*       let r2  = (b2 + r1) / pow2 51 in *)
-(*       let r3  = (b3 + r2) / pow2 51 in *)
-(*       v (get h1 b 5) = (b4 + r3) / pow2 51 *)
-(*       /\ v (get h1 b 0) = b0 % pow2 51 *)
-(*       /\ v (get h1 b 1) = (b1 + r0)  % pow2 51 *)
-(*       /\ v (get h1 b 2) = (b2 + r1)  % pow2 51 *)
-(*       /\ v (get h1 b 3) = (b3 + r2)  % pow2 51 *)
-(*       /\ v (get h1 b 4) = (b4 + r3)  % pow2 51 *)
-(*     ) *)
-
-let u633 = x:s64{H64.v x < pow2 63}
-
-(* let bound63 (h:heap) (b:bigint) : GTot Type0 = *)
-(*   live h b *)
-(*   /\ v (get h b 0) < pow2 63 /\ v (get h b 1) < pow2 63 /\ v (get h b 2) < pow2 63 *)
-(*   /\ v (get h b 3) < pow2 63 /\ v (get h b 4) < pow2 63 *)
-
 private val carry_1_0':
   b:bigint{length b >= norm_length+1} ->
-  b0:u633 -> b1:u633 -> b2:u633 -> b3:u633 -> b4:u633 ->
+  b0:H64.t -> b1:H64.t -> b2:H64.t -> b3:H64.t -> b4:H64.t ->
   Stack unit
-    (requires (fun h -> bound63 h b))
-    (ensures (fun h0 _ h1 -> bound63 h0 b /\ norm h1 b /\ modifies_1 b h0 h1
-      /\ isCarried_ h1 b0 b1 b2 b3 b4 b ))
+    (requires (fun h -> live h b))
+    (ensures (fun h0 _ h1 -> live h1 b /\ modifies_1 b h0 h1))
 let carry_1_0' b b0 b1 b2 b3 b4 =
-  assert_norm (pow2 51 = 2251799813685248);
-  assert_norm (pow2 13 = 8192);
-  assert_norm (pow2 63 = 9223372036854775808);
-  pow2_double_sum 63;
-  (* pow2_lt_compat 14 13; pow2_lt_compat 63 14; pow2_double_sum 63; *)
-  assert(forall x y. {:pattern (v x + v y)}(v x < pow2 63 /\ v y <= pow2 13)
-    ==> v x + v y < pow2 64);
   let b0' = mod_2_51 b0 in
   let r0  = div_2_51 b0 in
-  let b1' = mod_2_51 (b1 +^ r0) in
-  let r1  = div_2_51 (b1 +^ r0) in
-  let b2' = mod_2_51 (b2 +^ r1) in
-  let r2  = div_2_51 (b2 +^ r1) in
-  let b3' = mod_2_51 (b3 +^ r2) in
-  let r3  = div_2_51 (b3 +^ r2) in
-  let b4' = mod_2_51 (b4 +^ r3) in
-  let b5' = div_2_51 (b4 +^ r3) in
+  let b1' = mod_2_51 (b1 +%^ r0) in
+  let r1  = div_2_51 (b1 +%^ r0) in
+  let b2' = mod_2_51 (b2 +%^ r1) in
+  let r2  = div_2_51 (b2 +%^ r1) in
+  let b3' = mod_2_51 (b3 +%^ r2) in
+  let r3  = div_2_51 (b3 +%^ r2) in
+  let b4' = mod_2_51 (b4 +%^ r3) in
+  let b5' = div_2_51 (b4 +%^ r3) in
   update_6 b b0' b1' b2' b3' b4' b5'
 
 
@@ -413,9 +263,8 @@ let carry_1_0' b b0 b1 b2 b3 b4 =
 private val carry_1_':
   b:bigint{length b >= norm_length+1} ->
   Stack unit
-    (requires (fun h -> bound63 h b))
-    (ensures (fun h0 _ h1 -> bound63 h0 b /\ norm h1 b /\ modifies_1 b h0 h1
-      /\ isCarried h0 h1 b))
+    (requires (fun h -> live h b))
+    (ensures (fun h0 _ h1 -> live h1 b /\ modifies_1 b h0 h1))
 let carry_1_' b =
   let b0 = b.(0ul) in
   let b1 = b.(1ul) in
@@ -425,179 +274,93 @@ let carry_1_' b =
   carry_1_0' b b0 b1 b2 b3 b4
 
 
-(* let carried_1 (h:mem) (b:bigint) : GTot Type0 = *)
-(*   live h b /\ length b >= norm_length+1 *)
-(*   /\ v (get h b 0) < pow2 51 *)
-(*   /\ v (get h b 1) < pow2 51 *)
-(*   /\ v (get h b 2) < pow2 51 *)
-(*   /\ v (get h b 3) < pow2 51 *)
-(*   /\ v (get h b 4) < pow2 51 *)
-(*   /\ v (get h b 5) <= pow2 77 *)
-
 val carry_1':
   b:bigint{length b >= norm_length+1} ->
   Stack unit
-    (requires (fun h -> bound63 h b))
-    (ensures (fun h0 _ h1 -> bound63 h0 b /\ norm h1 b /\ modifies_1 b h0 h1
-      /\ eval h1 b (norm_length+1) = eval h0 b norm_length /\ carried_1 h1 b))
+    (requires (fun h -> live h b))
+    (ensures (fun h0 _ h1 -> live h1 b /\ modifies_1 b h0 h1))
 let carry_1' b =
-  let h0 = ST.get() in
-  carry_1_' b;
-  let h1 = ST.get() in
-  lemma_carry_1 h0 h1 b
-
-
-(* let carried_2 (h:mem) (b:bigint) : GTot Type0 = *)
-(*   live h b /\ length b >= norm_length+1 *)
-(*   /\ v (get h b 0) < pow2 84 *)
-(*   /\ v (get h b 1) < pow2 51 *)
-(*   /\ v (get h b 2) < pow2 51 *)
-(*   /\ v (get h b 3) < pow2 51 *)
-(*   /\ v (get h b 4) < pow2 51 *)
-
-val carry_2_':
-  b:bigint ->
-  Stack unit
-    (requires (fun h -> carried_2 h b))
-    (ensures (fun h0 _ h1 -> live h0 b /\ norm h1 b /\ modifies_1 b h0 h1
-      /\ isCarried h0 h1 b))
-let carry_2_' b =
-  pow2_lt_compat 63 52; pow2_lt_compat 63 51;
   carry_1_' b
 
 
-(* let carried_3 (h:mem) (b:bigint) : GTot Type0 = *)
-(*   norm h b /\ length b >= norm_length+1 *)
-(*   /\ v (get h b 5) <= 1 *)
-(*   /\ (v (get h b 5) = 1 *)
-(*       ==> (v (get h b 1) < pow2 16 /\ v (get h b 2) < pow2 16  /\ v (get h b 3) < pow2 16 *)
-(* 	  /\ v (get h b 4) < pow2 16)) *)
+val carry_2_':
+  b:bigint{length b >= norm_length + 1} ->
+  Stack unit
+    (requires (fun h -> live h b))
+    (ensures (fun h0 _ h1 -> live h1 b /\ modifies_1 b h0 h1))
+let carry_2_' b =
+  carry_1_' b
+
 
 val carry_2':
-  b:bigint ->
+  b:bigint{length b >= norm_length + 1} ->
   Stack unit
-    (requires (fun h -> carried_2 h b))
-    (ensures (fun h0 _ h1 -> carried_2 h0 b /\ norm h1 b /\ modifies_1 b h0 h1
-	  /\ eval h1 b (norm_length+1) = eval h0 b norm_length
-	  /\ carried_3 h1 b))
+    (requires (fun h -> live h b))
+    (ensures (fun h0 _ h1 -> live h1 b /\ modifies_1 b h0 h1))
 let carry_2' b =
-  let h0 = ST.get() in
-  carry_2_' b;
-  let h1 = ST.get() in
-  lemma_carry_2 h0 h1 b
+  carry_2_' b
 
-
-(* let carriedTopBottom (h0:mem) (h1:mem) (b:bigint) : GTot Type0 = *)
-(*   live h0 b /\ live h1 b /\ length b >= norm_length+1 *)
-(*   /\ v (get h1 b 0) = v (get h0 b 0) + 19 * v (get h0 b 5) *)
-(*   /\ v (get h1 b 1) = v (get h0 b 1) *)
-(*   /\ v (get h1 b 2) = v (get h0 b 2) *)
-(*   /\ v (get h1 b 3) = v (get h0 b 3) *)
-(*   /\ v (get h1 b 4) = v (get h0 b 4) *)
 
 val carry_top_':
-  b:bigint ->
+  b:bigint{length b >= norm_length + 1} ->
   Stack unit
-    (requires (fun h -> live h b /\ length b >= norm_length+1
-      /\ v (get h b 0) + 19 * v (get h b 5) < pow2 64 ))
-    (ensures  (fun h0 _ h1 -> live h1 b /\ modifies_1 b h0 h1
-      /\ carriedTopBottom h0 h1 b))
+    (requires (fun h -> live h b))
+    (ensures  (fun h0 _ h1 -> live h1 b /\ modifies_1 b h0 h1))
 let carry_top_' b =
   let b0 = b.(0ul) in
   let b5 = b.(5ul) in
-  b.(0ul) <- b0 +^ times_19 b5
+  b.(0ul) <- b0 +%^ times_19 b5
 
 
 val carry_top_1':
-  b:bigint ->
+  b:bigint{length b >= norm_length + 1} ->
   Stack unit
-    (requires (fun h -> carried_1 h b))
-    (ensures  (fun h0 _ h1 -> carried_1 h0 b /\ carried_2 h1 b /\ modifies_1 b h0 h1
-      /\ eval h1 b norm_length % reveal prime = eval h0 b (norm_length+1) % reveal prime))
+    (requires (fun h -> live h b))
+    (ensures  (fun h0 _ h1 -> live h1 b /\ modifies_1 b h0 h1))
 let carry_top_1' b =
-  let h0 = ST.get() in
-  assert_norm (pow2 13 = 8192);
-  assert_norm (pow2 51 = 2251799813685248);
-  assert_norm (pow2 63 = 9223372036854775808);
-  pow2_double_sum 51; pow2_double_sum 64;
-  carry_top_' b;
-  let h1 = ST.get() in
-  lemma_carry_top_1 h0 h1 b
+  carry_top_' b
 
-
-(* let carried_4 (h:mem) (b:bigint) : GTot Type0 = *)
-(*   live h b *)
-(*   /\ v (get h b 0) < pow2 51 + 19 *)
-(*   /\ v (get h b 1) < pow2 51 *)
-(*   /\ (v (get h b 0) >= pow2 51 ==> v (get h b 1) < pow2 16 // TODO: fix constant) *)
-(*   /\ v (get h b 2) < pow2 51 *)
-(*   /\ v (get h b 3) < pow2 51 *)
-(*   /\ v (get h b 4) < pow2 51) *)
 
 val carry_top_2':
-  b:bigint ->
+  b:bigint{length b >= norm_length + 1} ->
   Stack unit
-    (requires (fun h -> carried_3 h b))
-    (ensures  (fun h0 _ h1 -> carried_3 h0 b /\ carried_4 h1 b /\ modifies_1 b h0 h1
-      /\ eval h1 b norm_length % reveal prime = eval h0 b (norm_length+1) % reveal prime))
+    (requires (fun h -> live h b))
+    (ensures  (fun h0 _ h1 -> live h1 b /\ modifies_1 b h0 h1))
 let carry_top_2' b =
-  let h0 = ST.get() in
-  assert_norm (pow2 13 = 8192);
-  assert_norm (pow2 51 = 2251799813685248);
-  assert_norm (pow2 63 = 9223372036854775808);
-  pow2_double_sum 51; pow2_double_sum 64;
-  carry_top_' b;
-  let h1 = ST.get() in
-  lemma_carry_top_2 h0 h1 b
+  carry_top_' b
 
-
-(* let isCarried01 (h0:mem) (h1:mem) (b:bigint) = *)
-(*   live h0 b /\ live h1 b *)
-(*   /\ v (get h1 b 0) = v (get h0 b 0) % pow2 51 *)
-(*   /\ v (get h1 b 1) = v (get h0 b 1) + (v (get h0 b 0) / pow2 51) *)
-(*   /\ v (get h1 b 2) = v (get h0 b 2) *)
-(*   /\ v (get h1 b 3) = v (get h0 b 3) *)
-(*   /\ v (get h1 b 4) = v (get h0 b 4) *)
 
 
 #reset-options "--z3timeout 20 --initial_fuel 0 --max_fuel 0"
 
 private val carry_0_to_1_':
-  b:bigint ->
+  b:bigint{length b >= norm_length + 1} ->
   Stack unit
-    (requires (fun h -> carried_4 h b))
-    (ensures  (fun h0 _ h1 -> isCarried01 h0 h1 b /\ modifies_1 b h0 h1))
+    (requires (fun h -> live h b))
+    (ensures  (fun h0 _ h1 -> live h1 b /\ modifies_1 b h0 h1))
 let carry_0_to_1_' b =
-  assert_norm (pow2 0 = 1); assert_norm (pow2 1 = 2); assert_norm (pow2 2 = 4);
-  assert_norm (pow2 3 = 8); assert_norm (pow2 5 = 32);
-  pow2_lt_compat 63 5; pow2_lt_compat 63 51; pow2_double_sum 63;
   let b0 = b.(0ul) in
   let b1 = b.(1ul) in
   let b0' = mod_2_51 b0 in
   let r0  = div_2_51 b0 in
   b.(0ul) <- b0';
-  b.(1ul) <- b1 +^ r0
+  b.(1ul) <- b1 +%^ r0
 
 
 val carry_0_to_1':
-  b:bigint ->
+  b:bigint{length b >= norm_length + 1} ->
   Stack unit
-    (requires (fun h -> carried_4 h b))
-    (ensures  (fun h0 _ h1 -> carried_4 h0 b /\ modifies_1 b h0 h1 /\ norm h1 b
-      /\ eval h1 b norm_length = eval h0 b norm_length))
+    (requires (fun h -> live h b))
+    (ensures  (fun h0 _ h1 -> modifies_1 b h0 h1 /\ live h1 b))
 let carry_0_to_1' b =
-  let h0 = ST.get() in
-  carry_0_to_1_' b;
-  let h1 = ST.get() in
-  lemma_carry_0_to_1 h0 h1 b
+  carry_0_to_1_' b
 
 
 val freduce_coefficients:
   b:bigint{length b >= norm_length + 1} ->
   Stack unit
-    (requires (fun h -> bound63 h b))
-    (ensures (fun h0 _ h1 -> bound63 h0 b /\ norm h1 b /\ modifies_1 b h0 h1
-      /\ eval h1 b norm_length % reveal prime = eval h0 b norm_length % reveal prime))
+    (requires (fun h -> live h b))
+    (ensures (fun h0 _ h1 -> live h1 b /\ modifies_1 b h0 h1))
 let freduce_coefficients b =
   carry_1' b;
   carry_top_1' b;
@@ -605,80 +368,17 @@ let freduce_coefficients b =
   carry_top_2' b;
   carry_0_to_1' b
 
-  (* let m51 = 0x7ffffffffffffuL in *)
-  (* let b0 = b.(0ul) in *)
-  (* let b1 = b.(1ul) in *)
-  (* let b2 = b.(2ul) in *)
-  (* let b3 = b.(3ul) in *)
-  (* let b4 = b.(4ul) in *)
-  (* let r0 = b0 >>^ 51ul in *)
-  (* let b0 = b0 &^ m51 in *)
-  (* let b1 = b1 +^ r0 in *)
-  (* let r1 = b1 >>^ 51ul in *)
-  (* let b1 = b1 &^ m51 in *)
-  (* let b2 = b2 +^ r1 in *)
-  (* let r2 = b2 >>^ 51ul in *)
-  (* let b2 = b2 &^ m51 in *)
-  (* let b3 = b3 +^ r2 in *)
-  (* let r3 = b3 >>^ 51ul in *)
-  (* let b3 = b3 &^ m51 in *)
-  (* let b4 = b4 +^ r3 in *)
-  (* let r4 = b4 >>^ 51ul in *)
-  (* let b4 = b4 &^ m51 in *)
-  (* let r4 = r4 *^ 19uL in *)
-
-  (* let b0 = b0 +^ r4 in *)
-  (* let r0 = b0 >>^ 51ul in *)
-  (* let b0 = b0 &^ m51 in *)
-  (* let b1 = b1 +^ r0 in *)
-  (* let r1 = b1 >>^ 51ul in *)
-  (* let b1 = b1 &^ m51 in *)
-  (* let b2 = b2 +^ r1 in *)
-  (* let r2 = b2 >>^ 51ul in *)
-  (* let b2 = b2 &^ m51 in *)
-  (* let b3 = b3 +^ r2 in *)
-  (* let r3 = b3 >>^ 51ul in *)
-  (* let b3 = b3 &^ m51 in *)
-  (* let b4 = b4 +^ r3 in *)
-  (* let r4 = b4 >>^ 51ul in *)
-  (* let b4 = b4 &^ m51 in *)
-  (* let r4 = r4 *^ 19uL in *)
-
-  (* let b0 = b0 +^ r4 in *)
-  (* let r0 = b0 >>^ 51ul in *)
-  (* let b0 = b0 &^ m51 in *)
-  (* let b1 = b1 +^ r0 in *)
-
-  (* b.(0ul) <- b0; *)
-  (* b.(1ul) <- b1; *)
-  (* b.(2ul) <- b2; *)
-  (* b.(3ul) <- b3; *)
-  (* b.(4ul) <- b4 *)
-
-#reset-options "--initial_fuel 0 --max_fuel 9 --z3timeout 20"
-
-open Hacl.EC.Curve25519.Bignum.Modulo.Lemmas3
-
-
-private val lemma_2_255m19_val: n:nat ->
-  Lemma (requires (n = 255))
-        (ensures  (pow2 255 - 19 = 57896044618658097711785492504343953926634992332820282019728792003956564819949))
-        [SMTPat (pow2 n - 19)]
-let lemma_2_255m19_val n = assert_norm (pow2 255 - 19 = 57896044618658097711785492504343953926634992332820282019728792003956564819949)
 
 #reset-options "--initial_fuel 0 --max_fuel 9 --z3timeout 100"
 
 val normalize:
   b:bigint ->
   Stack unit
-    (requires (fun h -> norm h b))
-    (ensures (fun h0 _ h1 -> norm h0 b /\ norm h1 b /\ modifies_1 b h0 h1
-      /\ eval h1 b 5 = eval h0 b 5 % (pow2 255 - 19) ))
+    (requires (fun h -> live h b))
+    (ensures (fun h0 _ h1 -> live h1 b /\ modifies_1 b h0 h1))
 let normalize b =
-  let h0 = ST.get() in
   let two51m1 = (Hacl.Cast.uint64_to_sint64 0x7ffffffffffffuL) in
   let two51m19 = (Hacl.Cast.uint64_to_sint64 0x7ffffffffffeduL) in
-  assert_norm (v two51m1 = pow2 51 - 1); assert_norm(v two51m19 = pow2 51 - 19);
   let b0 = b.(0ul) in
   let b1 = b.(1ul) in
   let b2 = b.(2ul) in
@@ -690,28 +390,15 @@ let normalize b =
   let mask2 = H64.eq_mask b2 two51m1 in
   let mask1 = H64.eq_mask b1 two51m1 in
   let mask0 = H64.gte_mask b0 two51m19 in
-  UInt.logand_lemma_1 (v mask4); UInt.logand_lemma_2 (v mask4);
-  UInt.logand_lemma_1 (v mask3); UInt.logand_lemma_2 (v mask3);
-  UInt.logand_lemma_1 (v mask2); UInt.logand_lemma_2 (v mask2);
-  UInt.logand_lemma_1 (v mask1); UInt.logand_lemma_2 (v mask1);
-  UInt.logand_lemma_1 (v mask0); UInt.logand_lemma_2 (v mask0);
   let mask  = mask4 &^ mask3 &^ mask2 &^ mask1 &^ mask0 in
-  cut (maskPrime mask b0 b1 b2 b3 b4);
-  UInt.logand_lemma_1 (v two51m19); UInt.logand_lemma_2 (v two51m19);
-  UInt.logand_lemma_1 (v b1); UInt.logand_lemma_2 (v b1);
-  UInt.logand_lemma_1 (v b2); UInt.logand_lemma_2 (v b2);
-  UInt.logand_lemma_1 (v b3); UInt.logand_lemma_2 (v b3);
-  UInt.logand_lemma_1 (v b4); UInt.logand_lemma_2 (v b4);
-  let b0' = (b0 -^ (two51m19 &^ mask)) in
-  let b1' = (b1 -^ (b1 &^ mask)) in
-  let b2' = (b2 -^ (b2 &^ mask)) in
-  let b3' =  (b3 -^ (b3 &^ mask)) in
-  let b4' =  (b4 -^ (b4 &^ mask)) in
-  cut(masked mask b0 b1 b2 b3 b4 b0' b1' b2' b3' b4');
+  let b0' = (b0 -%^ (two51m19 &^ mask)) in
+  let b1' = (b1 -%^ (b1 &^ mask)) in
+  let b2' = (b2 -%^ (b2 &^ mask)) in
+  let b3' =  (b3 -%^ (b3 &^ mask)) in
+  let b4' =  (b4 -%^ (b4 &^ mask)) in
   b.(0ul) <- b0';
   b.(1ul) <- b1';
   b.(2ul) <- b2';
   b.(3ul) <- b3';
-  b.(4ul) <- b4';
-  let h1 = ST.get() in
-  lemma_finalize h0 b h1 b mask
+  b.(4ul) <- b4'
+
