crypto/ec/Hacl.EC.Curve25519.Ladder.fst
@@ -31,17 +31,17 @@ module H64  = Hacl.UInt64
 module H128  = Hacl.UInt128
 
 // Will be specified using the bitwise operators' semantics
-val mk_mask: x:s8 -> Tot (y:s64(* {v y < pow2 platform_size /\ (Hacl.UInt8.v x = 0 ==> v y = 0) /\ (Hacl.UInt8.v x = 1 ==> v y = pow2 platform_size - 1)} *))
-let mk_mask x =
+inline_for_extraction val mk_mask: x:s8 -> Tot (y:s64)
+inline_for_extraction let mk_mask x =
   let y = Hacl.Cast.sint8_to_sint64 x in
   H64 (Hacl.Cast.uint64_to_sint64 0uL -%^ y)
 
-val nth_bit: byt:s8 -> idx:u32{U32.v idx < 8} -> Tot (b:s8(* {S8.logand (S8.shift_right byt (7ul-|idx)) (uint8_to_sint8 1uy) == b /\ (b == uint8_to_sint8 0uy \/ b == uint8_to_sint8 1uy) } *))
-let nth_bit byte idx =
+inline_for_extraction val nth_bit: byt:s8 -> idx:u32{U32.v idx < 8} -> Tot (b:s8)
+inline_for_extraction let nth_bit byte idx =
   let open Hacl.UInt8 in
   let bit = (byte >>^ (U32 (7ul -^ idx))) &^ (Hacl.Cast.uint8_to_sint8 1uy) in
-  (* and_one_lemma (S8.shift_right byte (7-idx)); *)
   bit
+
 
 type distinct2 (n:bytes) (p:point) =
   disjoint n (get_x p) /\ disjoint n (get_y p) /\ disjoint n (get_z p)
@@ -54,33 +54,15 @@ val small_step_exit:
   p_plus_q:point{distinct p_plus_q two_p /\ distinct p_plus_q two_p_plus_q /\ distinct p_plus_q p /\ same_frame_2 p p_plus_q} ->
   q:point{distinct q two_p /\ distinct q two_p_plus_q /\ distinct q p /\ distinct q p_plus_q} ->
   n:erased nat -> byte:s8 ->
-  scalar:erased nat(* {reveal n = reveal scalar * (pow2 8) + (S8.v byte / (pow2 (8-8)))} *) ->
+  scalar:erased nat ->
   Stack unit
-     (requires (fun h -> live h two_p /\ live h two_p_plus_q /\ live h p /\ live h q /\ live h p_plus_q
-       (* (live h two_p) /\ (live h two_p_plus_q) /\ (onCurve h p) /\ (onCurve h p_plus_q) /\ (onCurve h q) *)
-       (* /\ (nTimesQ n (pointOf h q) h p p_plus_q)  *)
-     ))
+     (requires (fun h -> live h two_p /\ live h two_p_plus_q /\ live h p /\ live h q /\ live h p_plus_q))
      (ensures (fun h0 _ h1 -> live h1 two_p /\ live h1 two_p_plus_q /\ live h1 p /\ live h1 p_plus_q
        /\ HS.modifies_one (frame_of p) h0 h1
-       /\ HS.modifies_ref (frame_of p) (refs two_p ++ refs two_p_plus_q (* ++ refs p ++ refs p_plus_q *)) h0 h1 ))
-       (* (onCurve h0 p) /\ (onCurve h0 p_plus_q) /\ (onCurve h0 q) *)
-       (* /\ (onCurve h1 two_p) /\ (onCurve h1 two_p_plus_q) /\ (live h1 p) /\ (live h1 p_plus_q) /\ (onCurve h1 q)  *)
-       (* /\ (modifies (refs two_p +++ refs two_p_plus_q +++ refs p +++ refs p_plus_q) h0 h1) *)
-       // Formula_0 replaces (scalar * pow2 8 + byte)
-       (* /\ (nTimesQ  (formula_0 scalar byte) (pointOf h0 q) h1 two_p two_p_plus_q) *)
+       /\ HS.modifies_ref (frame_of p) (refs two_p ++ refs two_p_plus_q) h0 h1 ))
 let small_step_exit pp ppq p pq q n byte scalar =
-  (* let h0 = ST.get() in *)
   Hacl.EC.Curve25519.PPoint.copy2 pp ppq p pq;
-  (* let h1 = ST.get() in *)
-  (* distinct_lemma q p; distinct_lemma q pq; distinct_lemma q pp; distinct_lemma q ppq; *)
-  (* let s = (erefs pp +*+ erefs ppq +*+ erefs p +*+ erefs pq) in *)
-  (* cut(modifies (reveal s) h0 h1); *)
-  (* ad(True /\ FStar.TSet.intersect (reveal s) (refs q) = !{}); *)
-  (* on_curve_lemma h0 h1 q (erefs pp +*+ erefs ppq +*+ erefs p +*+ erefs pq); *)
-  (* cut(onCurve h1 q);  *)
-  (* cut(nTimesQ (hide (reveal scalar * pow2 8 + (S8.v byte / pow2 (8-8)))) (pointOf h0 q) h0 p pq);  *)
   ()
-  (* helper_lemma_1 scalar byte *)
 
 let lemma_helper_0 r s h0 h1 h2 h3 : Lemma
   (requires (HS.modifies_ref r s h0 h1 /\ HS.modifies_ref r s h1 h2 /\ HS.modifies_ref r s h2 h3))
@@ -133,40 +115,23 @@ val small_step_core:
    two_p:point -> two_p_plus_q:point{distinct two_p two_p_plus_q /\ same_frame_2 two_p two_p_plus_q} ->
    p:point{distinct two_p p /\ distinct two_p_plus_q p /\ same_frame_2 two_p_plus_q p} ->
    p_plus_q:point{distinct two_p p_plus_q /\ distinct two_p_plus_q p_plus_q /\ distinct p_plus_q p /\ same_frame_2 p p_plus_q} ->
-   q:point{same_frame q /\ frame_of q <> frame_of p
-   (* distinct q two_p /\ distinct q two_p_plus_q /\ distinct q p /\ distinct q p_plus_q *)} ->
-   n:erased nat -> ctr:u32{U32.v ctr<8} -> byt:s8 -> scalar:erased nat(* {reveal n = reveal scalar * (pow2 (w ctr)) + (S8.v byt / (pow2 (8-w ctr)))} *) ->
+   q:point{same_frame q /\ frame_of q <> frame_of p} ->
+   n:erased nat -> ctr:u32{U32.v ctr<8} -> byt:s8 -> scalar:erased nat ->
    Stack unit
      (requires (fun h -> live h two_p /\ live h two_p_plus_q /\ live h p /\ live h q /\ live h p_plus_q))
      (ensures (fun h0 _ h1 -> live h1 two_p /\ live h1 two_p_plus_q /\ live h1 p /\ live h1 p_plus_q
        /\ HS.modifies_one (frame_of p) h0 h1
        /\ HS.modifies_ref (frame_of p) (refs two_p ++ refs two_p_plus_q ++ refs p ++ refs p_plus_q) h0 h1 ))
-     (* (requires (fun h ->  *)
-     (*   (live h two_p) /\ (live h two_p_plus_q) /\ (onCurve h p) /\ (onCurve h p_plus_q) /\ (onCurve h q) *)
-     (*   /\ (nTimesQ n (pointOf h q) h p p_plus_q)  *)
-     (* )) *)
-     (* (ensures (fun h0 _ h1 -> *)
-     (*   (onCurve h0 p) /\ (onCurve h0 p_plus_q) /\ (onCurve h0 q) *)
-     (*   /\ (onCurve h1 two_p) /\ (onCurve h1 two_p_plus_q) /\ (live h1 p) /\ (live h1 p_plus_q) /\ (onCurve h1 q)  *)
-     (*   (\* /\ (modifies (refs two_p +++ refs two_p_plus_q +++ refs p +++ refs p_plus_q) h0 h1) *\) *)
-     (*   // Formula_0 replaces (scalar * pow2 8 + byte) *)
-     (*   /\ (nTimesQ  (formula_2 (reveal n) (nth_bit byt ctr)) (pointOf h0 q) h1 two_p two_p_plus_q) *)
-     (* )) *)
 let small_step_core pp ppq p pq q n ctr b scalar =
-  (* distinct_commutative p pq; *)
   let bit = nth_bit b ctr in
   let mask = mk_mask bit in
-  (* cut (v mask = pow2 platform_size - 1 \/ v mask = 0);  *)
   let h0 = ST.get() in
   swap_conditional p pq mask;
   let h1 = ST.get() in
   lemma_helper_001 p pq pp ppq q h0 h1;
-  (* let h = ST.get() in *)
-  (* small_step_core_lemma_1 h0 h pp ppq p pq q; *)
   Hacl.EC.Curve25519.AddAndDouble.double_and_add pp ppq p pq q;
   let h2 = ST.get() in
   lemma_helper_02 (frame_of p) q h1 h2;
-  (* let h2 = ST.get() in *)
   swap_conditional pp ppq mask;
   let h3 = ST.get() in
   lemma_helper_001 pp ppq p pq q h2 h3;
@@ -175,22 +140,6 @@ let small_step_core pp ppq p pq q n ctr b scalar =
   lemma_helper_0 (frame_of p) (refs pp ++ refs ppq ++ refs p ++ refs pq) h0 h1 h2 h3;
   ()
 
-  (* lemma_5 scalar b ctr; *)
-  (* let h1 = ST.get() in *)
-  (* assert ((live h2 p) /\ (live h2 pq) /\ (onCurve h2 q));  *)
-  (* assert (onCurve h1 pp /\ onCurve h1 ppq);  *)
-  (* let set2 = (erefs pp +*+ erefs ppq +*+ erefs p +*+ erefs pq) in *)
-  (* let set21 = (erefs pp +*+ erefs ppq) in *)
-  (* assert(modifies (reveal set21) h2 h1);  *)
-  (* small_step_core_lemma_1 h2 h1 p pq pp ppq q;  *)
-  (* small_step_core_lemma_2 h0 h h2 h1 pp ppq p pq q;  *)
-  (* cut ( bit == uint8_to_sint8 0uy ==> ((pointOf h p) = (pointOf h0 p) /\ (pointOf h pq) = (pointOf h0 pq)) ); *)
-  (* cut ( bit == uint8_to_sint8 1uy ==> ((pointOf h pq) = (pointOf h0 p) /\ (pointOf h p) = (pointOf h0 pq)) ); *)
-  (* cut ( ((pointOf h2 pp) = (Math.Curve.add (pointOf h p) (pointOf h p)) /\ (pointOf h2 ppq) = (Math.Curve.add (pointOf h p) (pointOf h pq))) ); *)
-  (* cut (bit == uint8_to_sint8 0uy ==> ((pointOf h1 pp) = (pointOf h2 pp) /\ (pointOf h1 ppq) = (pointOf h2 ppq))); *)
-  (* cut (bit == uint8_to_sint8 1uy ==> ((pointOf h1 pp) = (pointOf h2 ppq) /\ (pointOf h1 ppq) = (pointOf h2 pp)));  *)
-  (* cut (nTimesQ n (pointOf h0 q) h0 p pq);  *)
-  (* small_step_core_lemma_3 h0 h h2 h1 pp ppq p pq q n ctr b scalar *)
 
 #reset-options "--initial_fuel 0  --max_fuel 0 --z3timeout 100"
 
@@ -199,46 +148,24 @@ val small_step: two_p:point -> two_p_plus_q:point{distinct two_p two_p_plus_q /\
    p_plus_q:point{distinct p_plus_q two_p /\ distinct p_plus_q two_p_plus_q /\ distinct p_plus_q p /\ same_frame_2 p p_plus_q} ->
    q:point{same_frame q /\ frame_of q <> frame_of p} ->
    n:erased nat -> ctr:u32{U32.v ctr<=8} -> b:s8 ->
-   scalar:erased nat(* {reveal n = reveal scalar * (pow2 (w ctr)) + (S8.v b / (pow2 (8-w ctr)))} *) -> Stack unit
+   scalar:erased nat -> Stack unit
      (requires (fun h -> live h two_p /\ live h two_p_plus_q /\ live h p /\ live h q /\ live h p_plus_q))
      (ensures (fun h0 _ h1 -> live h1 two_p /\ live h1 two_p_plus_q /\ live h1 p /\ live h1 p_plus_q
        /\ HS.modifies_one (frame_of p) h0 h1
        /\ HS.modifies_ref (frame_of p) (refs two_p ++ refs two_p_plus_q ++ refs p ++ refs p_plus_q) h0 h1 ))
-     (* (requires (fun h -> live h two_p /\ live h two_p_plus_q /\ onCurve h p /\ onCurve h p_plus_q *)
-     (*   /\ onCurve h q /\ nTimesQ n (pointOf h q) h p p_plus_q )) *)
-     (* (ensures (fun h0 _ h1 -> onCurve h0 p /\ onCurve h0 p_plus_q /\ onCurve h0 q *)
-     (*   /\ (live h1 two_p) /\ (live h1 two_p_plus_q) /\ (onCurve h1 p) /\ (onCurve h1 p_plus_q) /\ (onCurve h1 q) *)
-     (*   (\* /\ (modifies (refs two_p +++ refs two_p_plus_q +++ refs p +++ refs p_plus_q) h0 h1) *\) *)
-     (*   // Formula_0 replaces (scalar * pow2 8 + b) *)
-     (*   /\ (nTimesQ  (formula_0 scalar b) (pointOf h0 q) h1 p p_plus_q) *)
-     (* )) *)
 let rec small_step pp ppq p pq q n ctr b scalar =
   if U32 (8ul =^ ctr) then begin
-    (* lemma_9 ctr; *)
-    (* helper_lemma_1 n b;  *)
     ()
   end
   else begin
     let h0 = ST.get() in
-    (* lemma_0 ctr 8; *)
     small_step_core pp ppq p pq q n ctr b scalar;
     let h1 = ST.get() in
     let bit = nth_bit b ctr in
-    (* cut (nTimesQ (formula_1 n bit) (pointOf h0 q) h1 pp ppq); *)
-    (* lemma_10 scalar ctr b; *)
-    // Replaces a missing definition of the euclidian division
-    (* admiP (True /\ 2*reveal n+S8.v bit = reveal scalar * (pow2 (w ctr+1)) + (S8.v b / pow2 (8 - (w ctr+1)))); *)
-    (* cut (w ctr+1 <= 8 /\ True); *)
-    (* assert (onCurve h1 pp /\ onCurve h1 ppq /\ live h1 p /\ live h1 pq); *)
     swap_both pp ppq p pq;
     let h2 = ST.get() in
-    (* assert (Math.Curve.equal (pointOf h2 p) (pointOf h1 pp) /\ Math.Curve.equal (pointOf h2 pq) (pointOf h1 ppq)); *)
-    (* small_step_lemma_1 h0 h1 h2 pp ppq p pq q; *)
-    (* formula_lemma n bit;  *)
-    (* assert(nTimesQ (eformula_2 n bit) (pointOf h2 q) h2 p pq); *)
-    small_step pp ppq p pq q (hide 0(* eformula_2 n bit *)) (U32 (ctr+^1ul)) b scalar;
+    small_step pp ppq p pq q (hide 0) (U32 (ctr+^1ul)) b scalar;
     let h3 = ST.get() in
-    (* small_step_lemma_2 h0 h1 h2 h3 pp ppq p pq q *)
     lemma_helper_0 (frame_of p) (refs pp ++ refs ppq ++ refs p ++ refs pq) h0 h1 h2 h3;
     ()
   end
@@ -262,30 +189,17 @@ val big_step:
     (ensures (fun h0 _ h1 -> live h1 pp /\ live h1 ppq /\ live h1 p /\ live h1 pq
        /\ HS.modifies_one (frame_of p) h0 h1
        /\ HS.modifies_ref (frame_of p) (refs pp ++ refs ppq ++ refs p ++ refs pq) h0 h1 ))
-    (* (requires (fun h -> live h pp /\ live h ppq /\ onCurve h p /\ onCurve h pq /\ onCurve h q *)
-    (*   /\ nTimesQ (formula_4 h n (w ctr)) (pointOf h q) h p pq )) *)
-    (* (ensures (fun h0 _ h1 -> live h0 pp /\ live h0 ppq /\ onCurve h0 p /\ onCurve h0 pq /\ onCurve h0 q *)
-    (*   /\ onCurve h1 p /\ onCurve h1 pq *)
-    (*   (\* /\ (modifies (refs pp +++ refs ppq +++ refs p +++ refs pq) h0 h1) *\) *)
-    (*   /\ nTimesQ (formula_4 h0 n (w ctr)) (pointOf h0 q) h0 p pq *)
-    (*   /\ nTimesQ (hide (valueOfBytes h0 n)) (pointOf h0 q) h1 p pq  )) *)
 let rec big_step n pp ppq p pq q ctr =
   let h0 = ST.get() in
-  if U32 (blength =^ ctr) then () (* assum(reveal (formula_4 h0 n bytes_length) = valueOfBytes h0 n) *)
+  if U32 (blength =^ ctr) then ()
   else begin
-    (* assum(bytes_length-1-w ctr>=0 /\ bytes_length-w ctr-1>=0); *)
     let byte = index n (U32 (blength-^1ul-^ctr)) in
-    (* let m = formula_4 h0 n (w ctr) in *)
-    // Replaces missing euclidian definitions in F*
-    (* admiP(reveal m = reveal m * pow2 0 + (S8.v byte / pow2 (8-0)) /\ True); *)
     small_step pp ppq p pq q (hide 0)(* m *) 0ul byte (hide 0)(* m *);
     let h1 = ST.get() in assert(live h1 q);
-    (* big_step_lemma_1 h0 h1 n pp ppq p pq q ctr byte; *)
     big_step n pp ppq p pq q (U32 (ctr +^ 1ul));
     let h2 = ST.get() in
     lemma_helper_1 (frame_of p) (refs pp ++ refs ppq ++ refs p ++ refs pq) h0 h1 h2;
     ()
-    (* big_step_lemma_2 h0 h1 h2 n pp ppq p pq q (w ctr) byte *)
   end
 
 #reset-options "--z3timeout 20 --initial_fuel 0 --max_fuel 0"
@@ -327,15 +241,10 @@ val montgomery_ladder:
   res:point{same_frame res} -> n:bytes{distinct2 n res /\ frame_of res <> frameOf n /\ length n >= 32} ->
   q:point{same_frame q /\ frame_of q <> frame_of res /\ frame_of q <> frameOf n} -> Stack unit
     (requires (fun h -> live h res /\ live h q /\ B.live h n))
-      (* live h res /\ onCurve h q )) *)
     (ensures (fun h0 _ h1 -> live h1 res
       /\ HS.modifies_one (frame_of res) h0 h1
       /\ HS.modifies_ref (frame_of res) (refs res) h0 h1
       /\ prop_2 h0 h1 res))
-    (* /\ modifies_3 (get_x res) (get_y res) (get_z res) h0 h1)) *)
-    (* live h0 res /\ onCurve h0 q /\ onCurve h1 res *)
-    (*   (\* /\ (modifies (refs res) h0 h1)  *\) *)
-    (*   /\ (pointOf h1 res = (valueOfBytes h0 n +* (pointOf h0 q)))  )) *)
 let montgomery_ladder res n q =
   let hinit = ST.get() in
   push_frame();
