crypto/symmetric/Hacl.Symmetric.Salsa20.fst
@@ -1,275 +1,1116 @@
 module Hacl.Symmetric.Salsa20
 
-open FStar.Mul
-open FStar.Ghost
+
 open FStar.HyperStack
 open FStar.ST
-open FStar.UInt32
 open FStar.Buffer
-
-open Hacl.UInt8
 open Hacl.UInt32
 open Hacl.Cast
 
-open Utils
 
-#reset-options "--max_fuel 0 --initial_fuel 0 --initial_ifuel 0 --max_ifuel 0 --z3timeout 5"
-
-(* Module abbreviations *)
-module HH = FStar.HyperHeap
-module HS = FStar.HyperStack
-
-module U8   = FStar.UInt8
-module U32  = FStar.UInt32
-module H8   = Hacl.UInt8
-module H32  = Hacl.UInt32
-module H64  = Hacl.UInt64
-
-(* This HAS to go in some more appropriate place *)
-assume MaxUInt32: pow2 32 = 4294967296
-
-(* Public machine integer types *)
-let u32 = U32.t
-let u8  = U8.t
-(* Secret machine integer types *)
-let h64 = H64.t
-let h32 = H32.t
-let h8  = H8.t
-
-let uint8_p = buffer H8.t
-let uint32_p = buffer H32.t
-let bytes = uint8_p
+let h32 = Hacl.UInt32.t
+let u32 = FStar.UInt32.t
+let uint8_p = buffer Hacl.UInt8.t
 
 
-(* Salsa 20 code *)
-val quarter_round:
-  m:uint32_p{length m = 16} ->
-  a:u32{FStar.UInt32.v a < 16} ->
-  b:u32{FStar.UInt32.v b<16} ->
-  c:u32{FStar.UInt32.v c<16} ->
-  d:u32{FStar.UInt32.v d<16} ->
+#reset-options "--initial_fuel 0 --max_fuel 0"
+
+private val lemma_max_uint32: n:nat -> Lemma
+  (requires (n = 32))
+  (ensures  (pow2 n = 4294967296))
+  [SMTPat (pow2 n)]
+let lemma_max_uint32 n = assert_norm(pow2 32 = 4294967296)
+private val lemma_max_uint64: n:nat -> Lemma
+  (requires (n = 64))
+  (ensures  (pow2 n = 18446744073709551616))
+  [SMTPat (pow2 n)]
+let lemma_max_uint64 n = assert_norm(pow2 64 = 18446744073709551616)
+
+
+let rotate (a:h32) (s:u32{FStar.UInt32.v s <= 32}) : Tot h32 =
+  (a <<^ s) |^ (a >>^ (FStar.UInt32 (32ul -^ s)))
+
+
+#reset-options "--initial_fuel 0 --max_fuel 0 --z3timeout 20"
+
+let load32_le (k:uint8_p) : Stack h32
+  (requires (fun h -> live h k /\ length k >= 4))
+  (ensures  (fun h0 _ h1 -> h0 == h1))
+  = let k0 = k.(0ul) in
+    let k1 = k.(1ul) in
+    let k2 = k.(2ul) in
+    let k3 = k.(3ul) in
+    let z = sint8_to_sint32 k0
+            |^ (sint8_to_sint32 k1 <<^ 8ul)
+            |^ (sint8_to_sint32 k2 <<^ 16ul)
+            |^ (sint8_to_sint32 k3 <<^ 24ul) in
+    z
+
+let store32_le (k:uint8_p) (x:h32) : Stack unit
+  (requires (fun h -> live h k /\ length k >= 4))
+  (ensures  (fun h0 _ h1 -> modifies_1 k h0 h1 /\ live h1 k))
+  = k.(0ul) <- sint32_to_sint8 x;
+    k.(1ul) <- sint32_to_sint8 (x >>^ 8ul);
+    k.(2ul) <- sint32_to_sint8 (x >>^ 16ul);
+    k.(3ul) <- sint32_to_sint8 (x >>^ 24ul)
+
+#reset-options "--initial_fuel 0 --max_fuel 0 --z3timeout 200"
+
+val crypto_core_salsa20:
+  output:uint8_p{length output = 64} ->
+  input :uint8_p{length input = 16} ->
+  key   :uint8_p{length key = 32} ->
   Stack unit
-    (requires (fun h -> live h m))
-    (ensures (fun h0 _ h1 -> live h1 m /\ modifies_1 m h0 h1))
-let quarter_round m a b c d =
-  let md = m.(d) in let mc = m.(c) in m.(a) <- m.(a) ^^ ((md +%^ mc) <<< 7ul);
-  let ma = m.(a) in let md = m.(d) in m.(b) <- m.(b) ^^ ((ma +%^ md) <<< 9ul);
-  let mb = m.(b) in let ma = m.(a) in m.(c) <- m.(c) ^^ ((mb +%^ ma) <<< 13ul);
-  let mc = m.(c) in let mb = m.(b) in m.(d) <- m.(d) ^^ ((mc +%^ mb) <<< 18ul)
+    (requires (fun h -> live h output /\ live h input /\ live h key))
+    (ensures  (fun h0 _ h1 -> modifies_1 output h0 h1 /\ live h1 output))
+let crypto_core_salsa20 output input key =
+  let x0 = uint32_to_sint32 0x61707865ul in
+  let x5 = uint32_to_sint32 0x3320646eul in
+  let x10 = uint32_to_sint32 0x79622d32ul in
+  let x15 = uint32_to_sint32 0x6b206574ul in
+  let x1 = load32_le(offset key 0ul) in
+  let x2 = load32_le(offset key 4ul) in
+  let x3 = load32_le(offset key 8ul) in
+  let x4 = load32_le(offset key 12ul) in
+  let x11 = load32_le(offset key 16ul) in
+  let x12 = load32_le(offset key 20ul) in
+  let x13 = load32_le(offset key 24ul) in
+  let x14 = load32_le(offset key 28ul) in
+  let x6 = load32_le(offset input 0ul) in
+  let x7 = load32_le(offset input 4ul) in
+  let x8 = load32_le(offset input 8ul) in
+  let x9 = load32_le(offset input 12ul) in
+  let j0 = x0 in
+  let j1 = x1 in
+  let j2 = x2 in
+  let j3 = x3 in
+  let j4 = x4 in
+  let j5 = x5 in
+  let j6 = x6 in
+  let j7 = x7 in
+  let j8 = x8 in
+  let j9 = x9 in
+  let j10 = x10 in
+  let j11 = x11 in
+  let j12 = x12 in
+  let j13 = x13 in
+  let j14 = x14 in
+  let j15 = x15 in
+  (* *)
+  let x4 = x4 ^^ rotate( x0+%^x12)  7ul in
+  let x8 = x8 ^^ rotate( x4+%^ x0)  9ul in
+  let x12 = x12 ^^ rotate( x8+%^ x4) 13ul in
+  let x0 = x0 ^^ rotate(x12+%^ x8) 18ul in
+  let x9 = x9 ^^ rotate( x5+%^ x1)  7ul in
+  let x13 = x13 ^^ rotate( x9+%^ x5)  9ul in
+  let x1 = x1 ^^ rotate(x13+%^ x9) 13ul in
+  let x5 = x5 ^^ rotate( x1+%^x13) 18ul in
+  let x14 = x14 ^^ rotate(x10+%^ x6)  7ul in
+  let x2 = x2 ^^ rotate(x14+%^x10)  9ul in
+  let x6 = x6 ^^ rotate( x2+%^x14) 13ul in
+  let x10 = x10 ^^ rotate( x6+%^ x2) 18ul in
+  let x3 = x3 ^^ rotate(x15+%^x11)  7ul in
+  let x7 = x7 ^^ rotate( x3+%^x15)  9ul in
+  let x11 = x11 ^^ rotate( x7+%^ x3) 13ul in
+  let x15 = x15 ^^ rotate(x11+%^ x7) 18ul in
+  let x1 = x1 ^^ rotate( x0+%^ x3)  7ul in
+  let x2 = x2 ^^ rotate( x1+%^ x0)  9ul in
+  let x3 = x3 ^^ rotate( x2+%^ x1) 13ul in
+  let x0 = x0 ^^ rotate( x3+%^ x2) 18ul in
+  let x6 = x6 ^^ rotate( x5+%^ x4)  7ul in
+  let x7 = x7 ^^ rotate( x6+%^ x5)  9ul in
+  let x4 = x4 ^^ rotate( x7+%^ x6) 13ul in
+  let x5 = x5 ^^ rotate( x4+%^ x7) 18ul in
+  let x11 = x11 ^^ rotate(x10+%^ x9)  7ul in
+  let x8 = x8 ^^ rotate(x11+%^x10)  9ul in
+  let x9 = x9 ^^ rotate( x8+%^x11) 13ul in
+  let x10 = x10 ^^ rotate( x9+%^ x8) 18ul in
+  let x12 = x12 ^^ rotate(x15+%^x14)  7ul in
+  let x13 = x13 ^^ rotate(x12+%^x15)  9ul in
+  let x14 = x14 ^^ rotate(x13+%^x12) 13ul in
+  let x15 = x15 ^^ rotate(x14+%^x13) 18ul in
+  (* *)
+  let x4 = x4 ^^ rotate( x0+%^x12)  7ul in
+  let x8 = x8 ^^ rotate( x4+%^ x0)  9ul in
+  let x12 = x12 ^^ rotate( x8+%^ x4) 13ul in
+  let x0 = x0 ^^ rotate(x12+%^ x8) 18ul in
+  let x9 = x9 ^^ rotate( x5+%^ x1)  7ul in
+  let x13 = x13 ^^ rotate( x9+%^ x5)  9ul in
+  let x1 = x1 ^^ rotate(x13+%^ x9) 13ul in
+  let x5 = x5 ^^ rotate( x1+%^x13) 18ul in
+  let x14 = x14 ^^ rotate(x10+%^ x6)  7ul in
+  let x2 = x2 ^^ rotate(x14+%^x10)  9ul in
+  let x6 = x6 ^^ rotate( x2+%^x14) 13ul in
+  let x10 = x10 ^^ rotate( x6+%^ x2) 18ul in
+  let x3 = x3 ^^ rotate(x15+%^x11)  7ul in
+  let x7 = x7 ^^ rotate( x3+%^x15)  9ul in
+  let x11 = x11 ^^ rotate( x7+%^ x3) 13ul in
+  let x15 = x15 ^^ rotate(x11+%^ x7) 18ul in
+  let x1 = x1 ^^ rotate( x0+%^ x3)  7ul in
+  let x2 = x2 ^^ rotate( x1+%^ x0)  9ul in
+  let x3 = x3 ^^ rotate( x2+%^ x1) 13ul in
+  let x0 = x0 ^^ rotate( x3+%^ x2) 18ul in
+  let x6 = x6 ^^ rotate( x5+%^ x4)  7ul in
+  let x7 = x7 ^^ rotate( x6+%^ x5)  9ul in
+  let x4 = x4 ^^ rotate( x7+%^ x6) 13ul in
+  let x5 = x5 ^^ rotate( x4+%^ x7) 18ul in
+  let x11 = x11 ^^ rotate(x10+%^ x9)  7ul in
+  let x8 = x8 ^^ rotate(x11+%^x10)  9ul in
+  let x9 = x9 ^^ rotate( x8+%^x11) 13ul in
+  let x10 = x10 ^^ rotate( x9+%^ x8) 18ul in
+  let x12 = x12 ^^ rotate(x15+%^x14)  7ul in
+  let x13 = x13 ^^ rotate(x12+%^x15)  9ul in
+  let x14 = x14 ^^ rotate(x13+%^x12) 13ul in
+  let x15 = x15 ^^ rotate(x14+%^x13) 18ul in
+  (* *)
+  let x4 = x4 ^^ rotate( x0+%^x12)  7ul in
+  let x8 = x8 ^^ rotate( x4+%^ x0)  9ul in
+  let x12 = x12 ^^ rotate( x8+%^ x4) 13ul in
+  let x0 = x0 ^^ rotate(x12+%^ x8) 18ul in
+  let x9 = x9 ^^ rotate( x5+%^ x1)  7ul in
+  let x13 = x13 ^^ rotate( x9+%^ x5)  9ul in
+  let x1 = x1 ^^ rotate(x13+%^ x9) 13ul in
+  let x5 = x5 ^^ rotate( x1+%^x13) 18ul in
+  let x14 = x14 ^^ rotate(x10+%^ x6)  7ul in
+  let x2 = x2 ^^ rotate(x14+%^x10)  9ul in
+  let x6 = x6 ^^ rotate( x2+%^x14) 13ul in
+  let x10 = x10 ^^ rotate( x6+%^ x2) 18ul in
+  let x3 = x3 ^^ rotate(x15+%^x11)  7ul in
+  let x7 = x7 ^^ rotate( x3+%^x15)  9ul in
+  let x11 = x11 ^^ rotate( x7+%^ x3) 13ul in
+  let x15 = x15 ^^ rotate(x11+%^ x7) 18ul in
+  let x1 = x1 ^^ rotate( x0+%^ x3)  7ul in
+  let x2 = x2 ^^ rotate( x1+%^ x0)  9ul in
+  let x3 = x3 ^^ rotate( x2+%^ x1) 13ul in
+  let x0 = x0 ^^ rotate( x3+%^ x2) 18ul in
+  let x6 = x6 ^^ rotate( x5+%^ x4)  7ul in
+  let x7 = x7 ^^ rotate( x6+%^ x5)  9ul in
+  let x4 = x4 ^^ rotate( x7+%^ x6) 13ul in
+  let x5 = x5 ^^ rotate( x4+%^ x7) 18ul in
+  let x11 = x11 ^^ rotate(x10+%^ x9)  7ul in
+  let x8 = x8 ^^ rotate(x11+%^x10)  9ul in
+  let x9 = x9 ^^ rotate( x8+%^x11) 13ul in
+  let x10 = x10 ^^ rotate( x9+%^ x8) 18ul in
+  let x12 = x12 ^^ rotate(x15+%^x14)  7ul in
+  let x13 = x13 ^^ rotate(x12+%^x15)  9ul in
+  let x14 = x14 ^^ rotate(x13+%^x12) 13ul in
+  let x15 = x15 ^^ rotate(x14+%^x13) 18ul in
+  (* *)
+  let x4 = x4 ^^ rotate( x0+%^x12)  7ul in
+  let x8 = x8 ^^ rotate( x4+%^ x0)  9ul in
+  let x12 = x12 ^^ rotate( x8+%^ x4) 13ul in
+  let x0 = x0 ^^ rotate(x12+%^ x8) 18ul in
+  let x9 = x9 ^^ rotate( x5+%^ x1)  7ul in
+  let x13 = x13 ^^ rotate( x9+%^ x5)  9ul in
+  let x1 = x1 ^^ rotate(x13+%^ x9) 13ul in
+  let x5 = x5 ^^ rotate( x1+%^x13) 18ul in
+  let x14 = x14 ^^ rotate(x10+%^ x6)  7ul in
+  let x2 = x2 ^^ rotate(x14+%^x10)  9ul in
+  let x6 = x6 ^^ rotate( x2+%^x14) 13ul in
+  let x10 = x10 ^^ rotate( x6+%^ x2) 18ul in
+  let x3 = x3 ^^ rotate(x15+%^x11)  7ul in
+  let x7 = x7 ^^ rotate( x3+%^x15)  9ul in
+  let x11 = x11 ^^ rotate( x7+%^ x3) 13ul in
+  let x15 = x15 ^^ rotate(x11+%^ x7) 18ul in
+  let x1 = x1 ^^ rotate( x0+%^ x3)  7ul in
+  let x2 = x2 ^^ rotate( x1+%^ x0)  9ul in
+  let x3 = x3 ^^ rotate( x2+%^ x1) 13ul in
+  let x0 = x0 ^^ rotate( x3+%^ x2) 18ul in
+  let x6 = x6 ^^ rotate( x5+%^ x4)  7ul in
+  let x7 = x7 ^^ rotate( x6+%^ x5)  9ul in
+  let x4 = x4 ^^ rotate( x7+%^ x6) 13ul in
+  let x5 = x5 ^^ rotate( x4+%^ x7) 18ul in
+  let x11 = x11 ^^ rotate(x10+%^ x9)  7ul in
+  let x8 = x8 ^^ rotate(x11+%^x10)  9ul in
+  let x9 = x9 ^^ rotate( x8+%^x11) 13ul in
+  let x10 = x10 ^^ rotate( x9+%^ x8) 18ul in
+  let x12 = x12 ^^ rotate(x15+%^x14)  7ul in
+  let x13 = x13 ^^ rotate(x12+%^x15)  9ul in
+  let x14 = x14 ^^ rotate(x13+%^x12) 13ul in
+  let x15 = x15 ^^ rotate(x14+%^x13) 18ul in
+  (* *)
+  let x4 = x4 ^^ rotate( x0+%^x12)  7ul in
+  let x8 = x8 ^^ rotate( x4+%^ x0)  9ul in
+  let x12 = x12 ^^ rotate( x8+%^ x4) 13ul in
+  let x0 = x0 ^^ rotate(x12+%^ x8) 18ul in
+  let x9 = x9 ^^ rotate( x5+%^ x1)  7ul in
+  let x13 = x13 ^^ rotate( x9+%^ x5)  9ul in
+  let x1 = x1 ^^ rotate(x13+%^ x9) 13ul in
+  let x5 = x5 ^^ rotate( x1+%^x13) 18ul in
+  let x14 = x14 ^^ rotate(x10+%^ x6)  7ul in
+  let x2 = x2 ^^ rotate(x14+%^x10)  9ul in
+  let x6 = x6 ^^ rotate( x2+%^x14) 13ul in
+  let x10 = x10 ^^ rotate( x6+%^ x2) 18ul in
+  let x3 = x3 ^^ rotate(x15+%^x11)  7ul in
+  let x7 = x7 ^^ rotate( x3+%^x15)  9ul in
+  let x11 = x11 ^^ rotate( x7+%^ x3) 13ul in
+  let x15 = x15 ^^ rotate(x11+%^ x7) 18ul in
+  let x1 = x1 ^^ rotate( x0+%^ x3)  7ul in
+  let x2 = x2 ^^ rotate( x1+%^ x0)  9ul in
+  let x3 = x3 ^^ rotate( x2+%^ x1) 13ul in
+  let x0 = x0 ^^ rotate( x3+%^ x2) 18ul in
+  let x6 = x6 ^^ rotate( x5+%^ x4)  7ul in
+  let x7 = x7 ^^ rotate( x6+%^ x5)  9ul in
+  let x4 = x4 ^^ rotate( x7+%^ x6) 13ul in
+  let x5 = x5 ^^ rotate( x4+%^ x7) 18ul in
+  let x11 = x11 ^^ rotate(x10+%^ x9)  7ul in
+  let x8 = x8 ^^ rotate(x11+%^x10)  9ul in
+  let x9 = x9 ^^ rotate( x8+%^x11) 13ul in
+  let x10 = x10 ^^ rotate( x9+%^ x8) 18ul in
+  let x12 = x12 ^^ rotate(x15+%^x14)  7ul in
+  let x13 = x13 ^^ rotate(x12+%^x15)  9ul in
+  let x14 = x14 ^^ rotate(x13+%^x12) 13ul in
+  let x15 = x15 ^^ rotate(x14+%^x13) 18ul in
+  (* *)
+  let x4 = x4 ^^ rotate( x0+%^x12)  7ul in
+  let x8 = x8 ^^ rotate( x4+%^ x0)  9ul in
+  let x12 = x12 ^^ rotate( x8+%^ x4) 13ul in
+  let x0 = x0 ^^ rotate(x12+%^ x8) 18ul in
+  let x9 = x9 ^^ rotate( x5+%^ x1)  7ul in
+  let x13 = x13 ^^ rotate( x9+%^ x5)  9ul in
+  let x1 = x1 ^^ rotate(x13+%^ x9) 13ul in
+  let x5 = x5 ^^ rotate( x1+%^x13) 18ul in
+  let x14 = x14 ^^ rotate(x10+%^ x6)  7ul in
+  let x2 = x2 ^^ rotate(x14+%^x10)  9ul in
+  let x6 = x6 ^^ rotate( x2+%^x14) 13ul in
+  let x10 = x10 ^^ rotate( x6+%^ x2) 18ul in
+  let x3 = x3 ^^ rotate(x15+%^x11)  7ul in
+  let x7 = x7 ^^ rotate( x3+%^x15)  9ul in
+  let x11 = x11 ^^ rotate( x7+%^ x3) 13ul in
+  let x15 = x15 ^^ rotate(x11+%^ x7) 18ul in
+  let x1 = x1 ^^ rotate( x0+%^ x3)  7ul in
+  let x2 = x2 ^^ rotate( x1+%^ x0)  9ul in
+  let x3 = x3 ^^ rotate( x2+%^ x1) 13ul in
+  let x0 = x0 ^^ rotate( x3+%^ x2) 18ul in
+  let x6 = x6 ^^ rotate( x5+%^ x4)  7ul in
+  let x7 = x7 ^^ rotate( x6+%^ x5)  9ul in
+  let x4 = x4 ^^ rotate( x7+%^ x6) 13ul in
+  let x5 = x5 ^^ rotate( x4+%^ x7) 18ul in
+  let x11 = x11 ^^ rotate(x10+%^ x9)  7ul in
+  let x8 = x8 ^^ rotate(x11+%^x10)  9ul in
+  let x9 = x9 ^^ rotate( x8+%^x11) 13ul in
+  let x10 = x10 ^^ rotate( x9+%^ x8) 18ul in
+  let x12 = x12 ^^ rotate(x15+%^x14)  7ul in
+  let x13 = x13 ^^ rotate(x12+%^x15)  9ul in
+  let x14 = x14 ^^ rotate(x13+%^x12) 13ul in
+  let x15 = x15 ^^ rotate(x14+%^x13) 18ul in
+  (* *)
+  let x4 = x4 ^^ rotate( x0+%^x12)  7ul in
+  let x8 = x8 ^^ rotate( x4+%^ x0)  9ul in
+  let x12 = x12 ^^ rotate( x8+%^ x4) 13ul in
+  let x0 = x0 ^^ rotate(x12+%^ x8) 18ul in
+  let x9 = x9 ^^ rotate( x5+%^ x1)  7ul in
+  let x13 = x13 ^^ rotate( x9+%^ x5)  9ul in
+  let x1 = x1 ^^ rotate(x13+%^ x9) 13ul in
+  let x5 = x5 ^^ rotate( x1+%^x13) 18ul in
+  let x14 = x14 ^^ rotate(x10+%^ x6)  7ul in
+  let x2 = x2 ^^ rotate(x14+%^x10)  9ul in
+  let x6 = x6 ^^ rotate( x2+%^x14) 13ul in
+  let x10 = x10 ^^ rotate( x6+%^ x2) 18ul in
+  let x3 = x3 ^^ rotate(x15+%^x11)  7ul in
+  let x7 = x7 ^^ rotate( x3+%^x15)  9ul in
+  let x11 = x11 ^^ rotate( x7+%^ x3) 13ul in
+  let x15 = x15 ^^ rotate(x11+%^ x7) 18ul in
+  let x1 = x1 ^^ rotate( x0+%^ x3)  7ul in
+  let x2 = x2 ^^ rotate( x1+%^ x0)  9ul in
+  let x3 = x3 ^^ rotate( x2+%^ x1) 13ul in
+  let x0 = x0 ^^ rotate( x3+%^ x2) 18ul in
+  let x6 = x6 ^^ rotate( x5+%^ x4)  7ul in
+  let x7 = x7 ^^ rotate( x6+%^ x5)  9ul in
+  let x4 = x4 ^^ rotate( x7+%^ x6) 13ul in
+  let x5 = x5 ^^ rotate( x4+%^ x7) 18ul in
+  let x11 = x11 ^^ rotate(x10+%^ x9)  7ul in
+  let x8 = x8 ^^ rotate(x11+%^x10)  9ul in
+  let x9 = x9 ^^ rotate( x8+%^x11) 13ul in
+  let x10 = x10 ^^ rotate( x9+%^ x8) 18ul in
+  let x12 = x12 ^^ rotate(x15+%^x14)  7ul in
+  let x13 = x13 ^^ rotate(x12+%^x15)  9ul in
+  let x14 = x14 ^^ rotate(x13+%^x12) 13ul in
+  let x15 = x15 ^^ rotate(x14+%^x13) 18ul in
+  (* *)
+  let x4 = x4 ^^ rotate( x0+%^x12)  7ul in
+  let x8 = x8 ^^ rotate( x4+%^ x0)  9ul in
+  let x12 = x12 ^^ rotate( x8+%^ x4) 13ul in
+  let x0 = x0 ^^ rotate(x12+%^ x8) 18ul in
+  let x9 = x9 ^^ rotate( x5+%^ x1)  7ul in
+  let x13 = x13 ^^ rotate( x9+%^ x5)  9ul in
+  let x1 = x1 ^^ rotate(x13+%^ x9) 13ul in
+  let x5 = x5 ^^ rotate( x1+%^x13) 18ul in
+  let x14 = x14 ^^ rotate(x10+%^ x6)  7ul in
+  let x2 = x2 ^^ rotate(x14+%^x10)  9ul in
+  let x6 = x6 ^^ rotate( x2+%^x14) 13ul in
+  let x10 = x10 ^^ rotate( x6+%^ x2) 18ul in
+  let x3 = x3 ^^ rotate(x15+%^x11)  7ul in
+  let x7 = x7 ^^ rotate( x3+%^x15)  9ul in
+  let x11 = x11 ^^ rotate( x7+%^ x3) 13ul in
+  let x15 = x15 ^^ rotate(x11+%^ x7) 18ul in
+  let x1 = x1 ^^ rotate( x0+%^ x3)  7ul in
+  let x2 = x2 ^^ rotate( x1+%^ x0)  9ul in
+  let x3 = x3 ^^ rotate( x2+%^ x1) 13ul in
+  let x0 = x0 ^^ rotate( x3+%^ x2) 18ul in
+  let x6 = x6 ^^ rotate( x5+%^ x4)  7ul in
+  let x7 = x7 ^^ rotate( x6+%^ x5)  9ul in
+  let x4 = x4 ^^ rotate( x7+%^ x6) 13ul in
+  let x5 = x5 ^^ rotate( x4+%^ x7) 18ul in
+  let x11 = x11 ^^ rotate(x10+%^ x9)  7ul in
+  let x8 = x8 ^^ rotate(x11+%^x10)  9ul in
+  let x9 = x9 ^^ rotate( x8+%^x11) 13ul in
+  let x10 = x10 ^^ rotate( x9+%^ x8) 18ul in
+  let x12 = x12 ^^ rotate(x15+%^x14)  7ul in
+  let x13 = x13 ^^ rotate(x12+%^x15)  9ul in
+  let x14 = x14 ^^ rotate(x13+%^x12) 13ul in
+  let x15 = x15 ^^ rotate(x14+%^x13) 18ul in
+  (* *)
+  let x4 = x4 ^^ rotate( x0+%^x12)  7ul in
+  let x8 = x8 ^^ rotate( x4+%^ x0)  9ul in
+  let x12 = x12 ^^ rotate( x8+%^ x4) 13ul in
+  let x0 = x0 ^^ rotate(x12+%^ x8) 18ul in
+  let x9 = x9 ^^ rotate( x5+%^ x1)  7ul in
+  let x13 = x13 ^^ rotate( x9+%^ x5)  9ul in
+  let x1 = x1 ^^ rotate(x13+%^ x9) 13ul in
+  let x5 = x5 ^^ rotate( x1+%^x13) 18ul in
+  let x14 = x14 ^^ rotate(x10+%^ x6)  7ul in
+  let x2 = x2 ^^ rotate(x14+%^x10)  9ul in
+  let x6 = x6 ^^ rotate( x2+%^x14) 13ul in
+  let x10 = x10 ^^ rotate( x6+%^ x2) 18ul in
+  let x3 = x3 ^^ rotate(x15+%^x11)  7ul in
+  let x7 = x7 ^^ rotate( x3+%^x15)  9ul in
+  let x11 = x11 ^^ rotate( x7+%^ x3) 13ul in
+  let x15 = x15 ^^ rotate(x11+%^ x7) 18ul in
+  let x1 = x1 ^^ rotate( x0+%^ x3)  7ul in
+  let x2 = x2 ^^ rotate( x1+%^ x0)  9ul in
+  let x3 = x3 ^^ rotate( x2+%^ x1) 13ul in
+  let x0 = x0 ^^ rotate( x3+%^ x2) 18ul in
+  let x6 = x6 ^^ rotate( x5+%^ x4)  7ul in
+  let x7 = x7 ^^ rotate( x6+%^ x5)  9ul in
+  let x4 = x4 ^^ rotate( x7+%^ x6) 13ul in
+  let x5 = x5 ^^ rotate( x4+%^ x7) 18ul in
+  let x11 = x11 ^^ rotate(x10+%^ x9)  7ul in
+  let x8 = x8 ^^ rotate(x11+%^x10)  9ul in
+  let x9 = x9 ^^ rotate( x8+%^x11) 13ul in
+  let x10 = x10 ^^ rotate( x9+%^ x8) 18ul in
+  let x12 = x12 ^^ rotate(x15+%^x14)  7ul in
+  let x13 = x13 ^^ rotate(x12+%^x15)  9ul in
+  let x14 = x14 ^^ rotate(x13+%^x12) 13ul in
+  let x15 = x15 ^^ rotate(x14+%^x13) 18ul in
+  (* *)
+  let x4 = x4 ^^ rotate( x0+%^x12)  7ul in
+  let x8 = x8 ^^ rotate( x4+%^ x0)  9ul in
+  let x12 = x12 ^^ rotate( x8+%^ x4) 13ul in
+  let x0 = x0 ^^ rotate(x12+%^ x8) 18ul in
+  let x9 = x9 ^^ rotate( x5+%^ x1)  7ul in
+  let x13 = x13 ^^ rotate( x9+%^ x5)  9ul in
+  let x1 = x1 ^^ rotate(x13+%^ x9) 13ul in
+  let x5 = x5 ^^ rotate( x1+%^x13) 18ul in
+  let x14 = x14 ^^ rotate(x10+%^ x6)  7ul in
+  let x2 = x2 ^^ rotate(x14+%^x10)  9ul in
+  let x6 = x6 ^^ rotate( x2+%^x14) 13ul in
+  let x10 = x10 ^^ rotate( x6+%^ x2) 18ul in
+  let x3 = x3 ^^ rotate(x15+%^x11)  7ul in
+  let x7 = x7 ^^ rotate( x3+%^x15)  9ul in
+  let x11 = x11 ^^ rotate( x7+%^ x3) 13ul in
+  let x15 = x15 ^^ rotate(x11+%^ x7) 18ul in
+  let x1 = x1 ^^ rotate( x0+%^ x3)  7ul in
+  let x2 = x2 ^^ rotate( x1+%^ x0)  9ul in
+  let x3 = x3 ^^ rotate( x2+%^ x1) 13ul in
+  let x0 = x0 ^^ rotate( x3+%^ x2) 18ul in
+  let x6 = x6 ^^ rotate( x5+%^ x4)  7ul in
+  let x7 = x7 ^^ rotate( x6+%^ x5)  9ul in
+  let x4 = x4 ^^ rotate( x7+%^ x6) 13ul in
+  let x5 = x5 ^^ rotate( x4+%^ x7) 18ul in
+  let x11 = x11 ^^ rotate(x10+%^ x9)  7ul in
+  let x8 = x8 ^^ rotate(x11+%^x10)  9ul in
+  let x9 = x9 ^^ rotate( x8+%^x11) 13ul in
+  let x10 = x10 ^^ rotate( x9+%^ x8) 18ul in
+  let x12 = x12 ^^ rotate(x15+%^x14)  7ul in
+  let x13 = x13 ^^ rotate(x12+%^x15)  9ul in
+  let x14 = x14 ^^ rotate(x13+%^x12) 13ul in
+  let x15 = x15 ^^ rotate(x14+%^x13) 18ul in
+  (* *)
+  let x0 = x0 +%^ j0 in
+  let x1 = x1 +%^ j1 in
+  let x2 = x2 +%^ j2 in
+  let x3 = x3 +%^ j3 in
+  let x4 = x4 +%^ j4 in
+  let x5 = x5 +%^ j5 in
+  let x6 = x6 +%^ j6 in
+  let x7 = x7 +%^ j7 in
+  let x8 = x8 +%^ j8 in
+  let x9 = x9 +%^ j9 in
+  let x10 = x10 +%^ j10 in
+  let x11 = x11 +%^ j11 in
+  let x12 = x12 +%^ j12 in
+  let x13 = x13 +%^ j13 in
+  let x14 = x14 +%^ j14 in
+  let x15 = x15 +%^ j15 in
+  (* *)
+  store32_le (offset output 0ul) x0;
+  store32_le (offset output 4ul) x1;
+  store32_le (offset output 8ul) x2;
+  store32_le (offset output 12ul) x3;
+  store32_le (offset output 16ul) x4;
+  store32_le (offset output 20ul) x5;
+  store32_le (offset output 24ul) x6;
+  store32_le (offset output 28ul) x7;
+  store32_le (offset output 32ul) x8;
+  store32_le (offset output 36ul) x9;
+  store32_le (offset output 40ul) x10;
+  store32_le (offset output 44ul) x11;
+  store32_le (offset output 48ul) x12;
+  store32_le (offset output 52ul) x13;
+  store32_le (offset output 56ul) x14;
+  store32_le (offset output 60ul) x15
 
 
-(* Salsa20 block function *)
-val double_round:
-  m:uint32_p{length m = 16} ->
+#reset-options "--initial_fuel 0 --max_fuel 0 --z3timeout 100"
+
+module U64 = FStar.UInt64
+module U32 = FStar.UInt32
+
+
+val xor_:
+  c:uint8_p{length c >= 64} ->
+  m:uint8_p{length m >= 64} ->
+  block:uint8_p{length block = 64} ->
   Stack unit
-    (requires (fun h -> live h m))
-    (ensures (fun h0 _ h1 -> live h1 m /\ modifies_1 m h0 h1 ))
-let double_round m =
-  quarter_round m  4ul  8ul 12ul  0ul;
-  quarter_round m  9ul 13ul  1ul  5ul;
-  quarter_round m 14ul  2ul  6ul 10ul;
-  quarter_round m  3ul  7ul 11ul 15ul;
-  quarter_round m  1ul  2ul  3ul  0ul;
-  quarter_round m  6ul  7ul  4ul  5ul;
-  quarter_round m 11ul  8ul  9ul 10ul;
-  quarter_round m 12ul 13ul 14ul 15ul
+    (requires (fun h -> live h c /\ live h m /\ live h block))
+    (ensures  (fun h0 _ h1 -> live h1 c /\ modifies_1 c h0 h1))
+let xor_ c m block =
+  let open Hacl.UInt8 in
+  let m0 = m.(0ul) in let block0 = block.(0ul) in
+  let m1 = m.(1ul) in let block1 = block.(1ul) in
+  let m2 = m.(2ul) in let block2 = block.(2ul) in
+  let m3 = m.(3ul) in let block3 = block.(3ul) in
+  let m4 = m.(4ul) in let block4 = block.(4ul) in
+  let m5 = m.(5ul) in let block5 = block.(5ul) in
+  let m6 = m.(6ul) in let block6 = block.(6ul) in
+  let m7 = m.(7ul) in let block7 = block.(7ul) in
+  let m8 = m.(8ul) in let block8 = block.(8ul) in
+  let m9 = m.(9ul) in let block9 = block.(9ul) in
+  let m10 = m.(10ul) in let block10 = block.(10ul) in
+  let m11 = m.(11ul) in let block11 = block.(11ul) in
+  let m12 = m.(12ul) in let block12 = block.(12ul) in
+  let m13 = m.(13ul) in let block13 = block.(13ul) in
+  let m14 = m.(14ul) in let block14 = block.(14ul) in
+  let m15 = m.(15ul) in let block15 = block.(15ul) in
+  let m16 = m.(16ul) in let block16 = block.(16ul) in
+  let m17 = m.(17ul) in let block17 = block.(17ul) in
+  let m18 = m.(18ul) in let block18 = block.(18ul) in
+  let m19 = m.(19ul) in let block19 = block.(19ul) in
+  let m20 = m.(20ul) in let block20 = block.(20ul) in
+  let m21 = m.(21ul) in let block21 = block.(21ul) in
+  let m22 = m.(22ul) in let block22 = block.(22ul) in
+  let m23 = m.(23ul) in let block23 = block.(23ul) in
+  let m24 = m.(24ul) in let block24 = block.(24ul) in
+  let m25 = m.(25ul) in let block25 = block.(25ul) in
+  let m26 = m.(26ul) in let block26 = block.(26ul) in
+  let m27 = m.(27ul) in let block27 = block.(27ul) in
+  let m28 = m.(28ul) in let block28 = block.(28ul) in
+  let m29 = m.(29ul) in let block29 = block.(29ul) in
+  let m30 = m.(30ul) in let block30 = block.(30ul) in
+  let m31 = m.(31ul) in let block31 = block.(31ul) in
+  let m32 = m.(32ul) in let block32 = block.(32ul) in
+  let m33 = m.(33ul) in let block33 = block.(33ul) in
+  let m34 = m.(34ul) in let block34 = block.(34ul) in
+  let m35 = m.(35ul) in let block35 = block.(35ul) in
+  let m36 = m.(36ul) in let block36 = block.(36ul) in
+  let m37 = m.(37ul) in let block37 = block.(37ul) in
+  let m38 = m.(38ul) in let block38 = block.(38ul) in
+  let m39 = m.(39ul) in let block39 = block.(39ul) in
+  let m40 = m.(40ul) in let block40 = block.(40ul) in
+  let m41 = m.(41ul) in let block41 = block.(41ul) in
+  let m42 = m.(42ul) in let block42 = block.(42ul) in
+  let m43 = m.(43ul) in let block43 = block.(43ul) in
+  let m44 = m.(44ul) in let block44 = block.(44ul) in
+  let m45 = m.(45ul) in let block45 = block.(45ul) in
+  let m46 = m.(46ul) in let block46 = block.(46ul) in
+  let m47 = m.(47ul) in let block47 = block.(47ul) in
+  let m48 = m.(48ul) in let block48 = block.(48ul) in
+  let m49 = m.(49ul) in let block49 = block.(49ul) in
+  let m50 = m.(50ul) in let block50 = block.(50ul) in
+  let m51 = m.(51ul) in let block51 = block.(51ul) in
+  let m52 = m.(52ul) in let block52 = block.(52ul) in
+  let m53 = m.(53ul) in let block53 = block.(53ul) in
+  let m54 = m.(54ul) in let block54 = block.(54ul) in
+  let m55 = m.(55ul) in let block55 = block.(55ul) in
+  let m56 = m.(56ul) in let block56 = block.(56ul) in
+  let m57 = m.(57ul) in let block57 = block.(57ul) in
+  let m58 = m.(58ul) in let block58 = block.(58ul) in
+  let m59 = m.(59ul) in let block59 = block.(59ul) in
+  let m60 = m.(60ul) in let block60 = block.(60ul) in
+  let m61 = m.(61ul) in let block61 = block.(61ul) in
+  let m62 = m.(62ul) in let block62 = block.(62ul) in
+  let m63 = m.(63ul) in let block63 = block.(63ul) in
+  c.(0ul) <- m0 ^^ block0;
+  c.(1ul) <- m1 ^^ block1;
+  c.(2ul) <- m2 ^^ block2;
+  c.(3ul) <- m3 ^^ block3;
+  c.(4ul) <- m4 ^^ block4;
+  c.(5ul) <- m5 ^^ block5;
+  c.(6ul) <- m6 ^^ block6;
+  c.(7ul) <- m7 ^^ block7;
+  c.(8ul) <- m8 ^^ block8;
+  c.(9ul) <- m9 ^^ block9;
+  c.(10ul) <- m10 ^^ block10;
+  c.(11ul) <- m11 ^^ block11;
+  c.(12ul) <- m12 ^^ block12;
+  c.(13ul) <- m13 ^^ block13;
+  c.(14ul) <- m14 ^^ block14;
+  c.(15ul) <- m15 ^^ block15;
+  c.(16ul) <- m16 ^^ block16;
+  c.(17ul) <- m17 ^^ block17;
+  c.(18ul) <- m18 ^^ block18;
+  c.(19ul) <- m19 ^^ block19;
+  c.(20ul) <- m20 ^^ block20;
+  c.(21ul) <- m21 ^^ block21;
+  c.(22ul) <- m22 ^^ block22;
+  c.(23ul) <- m23 ^^ block23;
+  c.(24ul) <- m24 ^^ block24;
+  c.(25ul) <- m25 ^^ block25;
+  c.(26ul) <- m26 ^^ block26;
+  c.(27ul) <- m27 ^^ block27;
+  c.(28ul) <- m28 ^^ block28;
+  c.(29ul) <- m29 ^^ block29;
+  c.(30ul) <- m30 ^^ block30;
+  c.(31ul) <- m31 ^^ block31;
+  c.(32ul) <- m32 ^^ block32;
+  c.(33ul) <- m33 ^^ block33;
+  c.(34ul) <- m34 ^^ block34;
+  c.(35ul) <- m35 ^^ block35;
+  c.(36ul) <- m36 ^^ block36;
+  c.(37ul) <- m37 ^^ block37;
+  c.(38ul) <- m38 ^^ block38;
+  c.(39ul) <- m39 ^^ block39;
+  c.(40ul) <- m40 ^^ block40;
+  c.(41ul) <- m41 ^^ block41;
+  c.(42ul) <- m42 ^^ block42;
+  c.(43ul) <- m43 ^^ block43;
+  c.(44ul) <- m44 ^^ block44;
+  c.(45ul) <- m45 ^^ block45;
+  c.(46ul) <- m46 ^^ block46;
+  c.(47ul) <- m47 ^^ block47;
+  c.(48ul) <- m48 ^^ block48;
+  c.(49ul) <- m49 ^^ block49;
+  c.(50ul) <- m50 ^^ block50;
+  c.(51ul) <- m51 ^^ block51;
+  c.(52ul) <- m52 ^^ block52;
+  c.(53ul) <- m53 ^^ block53;
+  c.(54ul) <- m54 ^^ block54;
+  c.(55ul) <- m55 ^^ block55;
+  c.(56ul) <- m56 ^^ block56;
+  c.(57ul) <- m57 ^^ block57;
+  c.(58ul) <- m58 ^^ block58;
+  c.(59ul) <- m59 ^^ block59;
+  c.(60ul) <- m60 ^^ block60;
+  c.(61ul) <- m61 ^^ block61;
+  c.(62ul) <- m62 ^^ block62;
+  c.(63ul) <- m63 ^^ block63
 
 
-(* 10 double rounds *)
-val rounds:
-  m:uint32_p{length m = 16} -> Stack unit
-    (requires (fun h -> live h m))
-    (ensures (fun h0 _ h1 -> live h1 m /\ modifies_1 m h0 h1 ))
-let rounds m =
-  double_round m;
-  double_round m;
-  double_round m;
-  double_round m;
-  double_round m;
-  double_round m;
-  double_round m;
-  double_round m;
-  double_round m;
-  double_round m
+#reset-options "--initial_fuel 0 --max_fuel 0 --z3timeout 100"
+
+let lemma_modifies_3 (c:uint8_p) (input:uint8_p) (block:uint8_p) h0 h1 h2 : Lemma
+  (requires (live h0 c /\ live h0 input /\ live h0 block
+    /\ live h1 c /\ live h1 input /\ live h1 block
+    /\ live h2 c /\ live h2 input /\ live h2 block
+    /\ modifies_2 c block h0 h1 /\ modifies_1 input h1 h2))
+  (ensures (modifies_3 c input block h0 h2))
+  = lemma_reveal_modifies_2 c block h0 h1;
+    lemma_reveal_modifies_1 input h1 h2;
+    lemma_intro_modifies_3 c input block h0 h2
 
 
-#reset-options "--max_fuel 0 --initial_fuel 0 --initial_ifuel 0 --max_ifuel 0"
+#reset-options "--initial_fuel 0 --max_fuel 0 --z3timeout 100"
 
-val initialize_state:
-  state:uint32_p{length state >= 16} ->
-  key:uint8_p{length key = 32 /\ disjoint state key} ->
-  counter:h64 ->
-  nonce:uint8_p{length nonce = 8 /\ disjoint state nonce} ->
+let lemma_modifies_3' (c:uint8_p) (input:uint8_p) (block:uint8_p) h0 h1 h2 : Lemma
+  (requires (live h0 c /\ live h0 input /\ live h0 block
+    /\ live h1 c /\ live h1 input /\ live h1 block
+    /\ live h2 c /\ live h2 input /\ live h2 block
+    /\ length c >= 64 /\ modifies_3 c input block h0 h1
+    /\ modifies_3 (offset c 64ul) input block h1 h2))
+  (ensures (modifies_3 c input block h0 h2))
+  = lemma_reveal_modifies_3 c input block h0 h1;
+    lemma_reveal_modifies_3 (offset c 64ul) input block h1 h2;
+    lemma_intro_modifies_3 c input block h0 h2
+
+
+#reset-options "--initial_fuel 0 --max_fuel 0 --z3timeout 100"
+
+val crypto_stream_salsa20_xor_ic_loop:
+  c:uint8_p ->
+  m:uint8_p ->
+  block:uint8_p{length block = 64 /\ disjoint block c} ->
+  input:uint8_p{length input = 16 /\ disjoint input block /\ disjoint input c} ->
+  kcopy:uint8_p{length kcopy = 32 /\ disjoint kcopy block} ->
+  mlen:FStar.UInt64.t{U64.v mlen <= length c /\ U64.v mlen <= length m} ->
+  Stack (z:FStar.UInt64.t{FStar.UInt64.v z < 64})
+    (requires (fun h -> live h c /\ live h m /\ live h block /\ live h input /\ live h kcopy))
+    (ensures  (fun h0 _ h1 -> live h1 c /\ live h1 input /\ live h1 block /\ modifies_3 c input block h0 h1))
+let rec crypto_stream_salsa20_xor_ic_loop c m block input kcopy mlen =
+  if (FStar.UInt64 (mlen <^ 64uL)) then (
+    let h = ST.get() in
+    lemma_intro_modifies_3 c input block h h;
+    mlen )
+  else (
+    let h0 = ST.get() in
+    let open Hacl.UInt8 in
+    crypto_core_salsa20 block input kcopy;
+    let h1 = ST.get() in cut (modifies_1 block h0 h1);
+    xor_ c m block;
+    let h2 = ST.get() in
+    (* *)
+    let i8 = input.(8ul) in
+    let i9 = input.(9ul) in
+    let i10 = input.(10ul) in
+    let i11 = input.(11ul) in
+    let i12 = input.(12ul) in
+    let i13 = input.(13ul) in
+    let i14 = input.(14ul) in
+    let i15 = input.(15ul) in
+    (* *)
+    let u = Hacl.UInt64(
+      sint8_to_sint64 i8
+      +%^ (sint8_to_sint64 i9 <<^ 8ul)
+      +%^ (sint8_to_sint64 i10 <<^ 16ul)
+      +%^ (sint8_to_sint64 i11 <<^ 24ul)
+      +%^ (sint8_to_sint64 i12 <<^ 32ul)
+      +%^ (sint8_to_sint64 i13 <<^ 40ul)
+      +%^ (sint8_to_sint64 i14 <<^ 48ul)
+      +%^ (sint8_to_sint64 i15 <<^ 56ul)
+      +%^ (uint64_to_sint64 1uL)
+    ) in
+    (* *)
+    cut (modifies_2 c block h0 h2);
+    input.(8ul)  <- sint64_to_sint8 u;
+    input.(9ul)  <- sint64_to_sint8 (Hacl.UInt64 (u >>^ 8ul));
+    input.(10ul) <- sint64_to_sint8 (Hacl.UInt64 (u >>^ 16ul));
+    input.(11ul) <- sint64_to_sint8 (Hacl.UInt64 (u >>^ 24ul));
+    input.(12ul) <- sint64_to_sint8 (Hacl.UInt64 (u >>^ 32ul));
+    input.(13ul) <- sint64_to_sint8 (Hacl.UInt64 (u >>^ 40ul));
+    input.(14ul) <- sint64_to_sint8 (Hacl.UInt64 (u >>^ 48ul));
+    input.(15ul) <- sint64_to_sint8 (Hacl.UInt64 (u >>^ 56ul));
+    (* *)
+    let h3 = ST.get() in
+    lemma_modifies_3 c input block h0 h2 h3;
+    let mlen = FStar.UInt64 (mlen -^ 64uL) in
+    let c' = offset c 64ul in
+    let m = offset m 64ul in
+    (* *)
+    let res = crypto_stream_salsa20_xor_ic_loop c' m block input kcopy mlen in
+    let h4 = ST.get() in
+    lemma_modifies_3' c input block h0 h3 h4;
+    res
+  )
+
+
+#reset-options "--initial_fuel 0 --max_fuel 0 --z3timeout 10"
+
+val xor_bytes:
+  x:uint8_p ->
+  y:uint8_p ->
+  z:uint8_p ->
+  len:FStar.UInt32.t{let l = U32.v len in length x >= l /\ length y >= l /\ length z >= l} ->
   Stack unit
-    (requires (fun h -> live h state /\ live h key /\ live h nonce))
-    (ensures (fun h0 _ h1 -> live h1 state /\ modifies_1 state h0 h1))
-let initialize_state state key counter nonce =
-  (* Key part *)
-  let open FStar.Buffer in // Shadowing the 'sub' definition
+    (requires (fun h -> live h x /\ live h y /\ live h z))
+    (ensures  (fun h0 _ h1 -> live h1 x /\ modifies_1 x h0 h1))
+let rec xor_bytes x y z len =
+  if FStar.UInt32 (len =^ 0ul) then ()
+  else (
+    let i = FStar.UInt32 (len -^ 1ul) in
+    let yi = y.(i) in let zi = z.(i) in
+    x.(i) <- Hacl.UInt8 (yi ^^ zi);
+    xor_bytes x y z i
+  )
+
+
+#reset-options "--initial_fuel 0 --max_fuel 0 --z3timeout 20"
+
+
+inline_for_extraction let mod_64 (mlen:U64.t) : Tot (z:U32.t{U32.v z = U64.v mlen % 64 /\ U32.v z <= U64.v mlen}) =
+  let mlen' = U64 (mlen &^ 63uL) in
+  UInt.logand_mask (U64.v mlen) 6;
+  assert_norm (pow2 6 = 64);
+  Math.Lemmas.euclidean_division_definition (U64.v mlen) 64;
+  Math.Lemmas.nat_over_pos_is_nat (U64.v mlen) 64;
+  Math.Lemmas.nat_times_nat_is_nat (U64.v mlen / 64) 64;
+  cut (U64 (v mlen >= v mlen'));
+  Math.Lemmas.modulo_lemma (U64.v mlen') (pow2 32);
+  Int.Cast.uint64_to_uint32 mlen'
+
+
+#reset-options "--initial_fuel 0 --max_fuel 0 --z3timeout 200"
+
+let lemma_modifies_3_1 (c:uint8_p) (input:uint8_p) (block:uint8_p) h0 h1 h2 h3 : Lemma
+  (requires (live h0 c /\ ~(contains h0 input) /\ ~(contains h0 block)
+    /\ live h1 c /\ live h1 input /\ live h1 block
+    /\ live h2 c /\ live h2 input /\ live h2 block
+    /\ live h3 c /\ live h3 input /\ live h3 block
+    /\ modifies_0 h0 h1 /\ modifies_3 c input block h1 h2 /\ modifies_2 c block h2 h3))
+  (ensures (modifies_2_1 c h0 h3))
+  = lemma_reveal_modifies_0 h0 h1;
+    lemma_reveal_modifies_3 c input block h1 h2;
+    lemma_reveal_modifies_2 c block h2 h3;
+    lemma_intro_modifies_2_1 c h0 h3
+
+
+#reset-options "--initial_fuel 0 --max_fuel 0 --z3timeout 50"
+
+val crypto_stream_salsa20_xor_ic__:
+  n:uint8_p{length n = 8} ->
+  ic:FStar.UInt64.t ->
+  k:uint8_p{length k = 32} ->
+  local_state:uint8_p{length local_state = 112} ->
+  Stack unit
+    (requires (fun h -> live h n /\ live h k /\ live h local_state))
+    (ensures  (fun h0 _ h1 -> live h1 local_state /\ modifies_1 local_state h0 h1))
+let crypto_stream_salsa20_xor_ic__ n ic k local_state =
+  let input = Buffer.sub local_state 0ul  16ul in
+  let block = Buffer.sub local_state 16ul 64ul in
+  let kcopy = Buffer.sub local_state 80ul 32ul in
+  let k0 = k.(0ul) in let k1 = k.(1ul) in let k2 = k.(2ul) in let k3 = k.(3ul) in
+  let k4 = k.(4ul) in let k5 = k.(5ul) in let k6 = k.(6ul) in let k7 = k.(7ul) in
+  let k8 = k.(8ul) in let k9 = k.(9ul) in let k10 = k.(10ul) in let k11 = k.(11ul) in
+  let k12 = k.(12ul) in let k13 = k.(13ul) in let k14 = k.(14ul) in let k15 = k.(15ul) in
+  let k16 = k.(16ul) in let k17 = k.(17ul) in let k18 = k.(18ul) in let k19 = k.(19ul) in
+  let k20 = k.(20ul) in let k21 = k.(21ul) in let k22 = k.(22ul) in let k23 = k.(23ul) in
+  let k24 = k.(24ul) in let k25 = k.(25ul) in let k26 = k.(26ul) in let k27 = k.(27ul) in
+  let k28 = k.(28ul) in let k29 = k.(29ul) in let k30 = k.(30ul) in let k31 = k.(31ul) in
+  let n0 = n.(0ul) in let n1 = n.(1ul) in let n2 = n.(2ul) in let n3 = n.(3ul) in
+  let n4 = n.(4ul) in let n5 = n.(5ul) in let n6 = n.(6ul) in let n7 = n.(7ul) in
+  kcopy.(0ul) <- k0;   kcopy.(1ul) <- k1;
+  kcopy.(2ul) <- k2;   kcopy.(3ul) <- k3;
+  kcopy.(4ul) <- k4;   kcopy.(5ul) <- k5;
+  kcopy.(6ul) <- k6;   kcopy.(7ul) <- k7;
+  kcopy.(8ul) <- k8;   kcopy.(9ul) <- k9;
+  kcopy.(10ul) <- k10; kcopy.(11ul) <- k11;
+  kcopy.(12ul) <- k12; kcopy.(13ul) <- k13;
+  kcopy.(14ul) <- k14; kcopy.(15ul) <- k15;
+  kcopy.(16ul) <- k16; kcopy.(17ul) <- k17;
+  kcopy.(18ul) <- k18; kcopy.(19ul) <- k19;
+  kcopy.(20ul) <- k20; kcopy.(21ul) <- k21;
+  kcopy.(22ul) <- k22; kcopy.(23ul) <- k23;
+  kcopy.(24ul) <- k24; kcopy.(25ul) <- k25;
+  kcopy.(26ul) <- k26; kcopy.(27ul) <- k27;
+  kcopy.(28ul) <- k28; kcopy.(29ul) <- k29;
+  kcopy.(30ul) <- k30; kcopy.(31ul) <- k31;
+  input.(0ul) <- n0;   input.(1ul) <- n1;
+  input.(2ul) <- n2;   input.(3ul) <- n3;
+  input.(4ul) <- n4;   input.(5ul) <- n5;
+  input.(6ul) <- n6;   input.(7ul) <- n7;
+  input.(8ul)  <- uint64_to_sint8 ic;
+  input.(9ul)  <- uint64_to_sint8 (FStar.UInt64 (ic >>^ 8ul));
+  input.(10ul) <- uint64_to_sint8 (FStar.UInt64 (ic >>^ 16ul));
+  input.(11ul) <- uint64_to_sint8 (FStar.UInt64 (ic >>^ 24ul));
+  input.(12ul) <- uint64_to_sint8 (FStar.UInt64 (ic >>^ 32ul));
+  input.(13ul) <- uint64_to_sint8 (FStar.UInt64 (ic >>^ 40ul));
+  input.(14ul) <- uint64_to_sint8 (FStar.UInt64 (ic >>^ 48ul));
+  input.(15ul) <- uint64_to_sint8 (FStar.UInt64 (ic >>^ 56ul))
+
+
+#reset-options "--initial_fuel 0 --max_fuel 0 --z3timeout 100"
+
+val crypto_stream_salsa20_xor_ic_:
+  c:uint8_p ->
+  m:uint8_p ->
+  mlen:FStar.UInt64.t{U64.v mlen <= length c /\ U64.v mlen <= length m /\ U64.v mlen > 0} ->
+  n:uint8_p{length n = 8} ->
+  ic:FStar.UInt64.t ->
+  k:uint8_p{length k = 32} ->
+  Stack unit
+    (requires (fun h -> live h c /\ live h m /\ live h n /\ live h k))
+    (ensures  (fun h0 _ h1 -> live h1 c /\ modifies_1 c h0 h1))
+let crypto_stream_salsa20_xor_ic_ c m mlen n ic k =
+  cut (U64.v mlen < pow2 32);
+  Math.Lemmas.modulo_lemma (U64.v mlen) (pow2 32);
+  push_frame();
   let h0 = ST.get() in
-  let k0 = sub key 0ul  4ul in
-  let k1 = sub key 4ul  4ul in
-  let k2 = sub key 8ul  4ul in
-  let k3 = sub key 12ul 4ul in
-  let k4 = sub key 16ul 4ul in
-  let k5 = sub key 20ul 4ul in
-  let k6 = sub key 24ul 4ul in
-  let k7 = sub key 28ul 4ul in
-  let k0 = (uint32_of_bytes k0) in
-  let k1 = (uint32_of_bytes k1) in
-  let k2 = (uint32_of_bytes k2) in
-  let k3 = (uint32_of_bytes k3) in
-  let k4 = (uint32_of_bytes k4) in
-  let k5 = (uint32_of_bytes k5) in
-  let k6 = (uint32_of_bytes k6) in
-  let k7 = (uint32_of_bytes k7) in
-  (* Nonce part *)
-  let n0 = sub nonce 0ul 4ul in
-  let n1 = sub nonce 4ul 4ul in
-  let n0 =  (uint32_of_bytes n0) in
-  let n1 =  (uint32_of_bytes n1) in
-  (* Constant part *)
-  state.(0ul) <-  (uint32_to_sint32 0x61707865ul);
-  state.(5ul) <-  (uint32_to_sint32 0x3320646eul);
-  state.(10ul) <- (uint32_to_sint32 0x79622d32ul);
-  state.(15ul) <- (uint32_to_sint32 0x6b206574ul);
-  (* Update with key *)
-  state.(1ul) <-  (k0);
-  state.(2ul) <-  (k1);
-  state.(3ul) <-  (k2);
-  state.(4ul) <-  (k3);
-  state.(11ul) <- (k4);
-  state.(12ul) <- (k5);
-  state.(13ul) <- (k6);
-  state.(14ul) <- (k7);
-  (* Update with nonces *)
-  state.(6ul) <- (n0);
-  state.(7ul) <- (n1);
-  (* Block counter part *)
-  let c0 = sint64_to_sint32 counter in
-  let c1 = sint64_to_sint32 (H64 (counter >>^ 32ul)) in
-  state.(8ul) <- c0;
-  state.(9ul) <- c1
-
-
-val salsa20_core:
-  output:uint8_p ->
-  state:uint32_p{length state >= 32 /\ disjoint state output} ->
-  key:uint8_p{length key = 32 /\ disjoint state key /\ disjoint output key} ->
-  counter:h64 ->
-  nonce:uint8_p{length nonce = 8 /\ disjoint state nonce /\ disjoint output nonce} ->
-  len:u32{FStar.UInt32.v len <= 64 /\ length output >= FStar.UInt32.v len} ->
-  Stack unit
-    (requires (fun h -> live h state /\ live h output /\ live h key /\ live h nonce))
-    (ensures (fun h0 _ h1 -> live h1 output /\ live h1 state /\ modifies_2 output state h0 h1 ))
-let salsa20_core output state key counter nonce len =
-  let open FStar.Buffer in // local shadowing of the 'sub' definition
-  (* Initialize internal state *)
-  let m = sub state 0ul 16ul in
-  let m0 = sub state 16ul 16ul in
-  initialize_state m key counter nonce;
-  (* Initial state *)
-  blit m 0ul m0 0ul 16ul;
-  (* 20 rounds *)
-  rounds m;
-  (* Sum the matrixes *)
-  sum_matrixes m m0;
-  (* Serialize the state into byte stream *)
-  bytes_of_uint32s output m len
-
-
-val salsa20_encrypt_loop:
-  state:uint32_p{length state >= 32} ->
-  key:uint8_p{length key = 32 /\ disjoint state key} ->
-  counter:h64 ->
-  nonce:uint8_p{length nonce = 8 /\ disjoint state nonce} ->
-  plaintext:uint8_p{disjoint state plaintext} ->
-  ciphertext:uint8_p{disjoint state ciphertext /\ disjoint key ciphertext /\ disjoint nonce ciphertext /\ disjoint plaintext ciphertext} ->
-  j:u32 ->
-  max:u32{FStar.UInt32.v j <= FStar.UInt32.v max /\ Hacl.UInt64.v counter + FStar.UInt32.v max < pow2 n} ->
-  Stack unit
-    (requires (fun h -> live h state /\ live h key /\ live h nonce /\ live h plaintext  /\ live h ciphertext
-      /\ length plaintext >= (FStar.UInt32.v max-FStar.UInt32.v j) * 64  /\ length ciphertext >= (FStar.UInt32.v max-FStar.UInt32.v j) * 64 ))
-    (ensures (fun h0 _ h1 -> live h1 ciphertext /\ live h1 state /\ modifies_2 ciphertext state h0 h1 ))
-let rec salsa20_encrypt_loop state key counter nonce plaintext ciphertext j max =
-  if j =^ max then ()
-  else
-    begin
-      (* Generate new state for block *)
-      let open FStar.Buffer in
-      let cipher_block = sub ciphertext 0ul 64ul in
-      let ciphertext' = sub ciphertext 64ul (U32 (64ul *^ (max -^ j -^ 1ul))) in
-      let plain_block = sub plaintext 0ul 64ul in
-      let plaintext' = sub plaintext 64ul (U32 (64ul *^ (max -^ j -^ 1ul))) in
-      salsa20_core cipher_block state key (H64 (counter +^ (uint32_to_sint64 j))) nonce 64ul;
-      (* XOR the key stream with the plaintext *)
-      xor_uint8_p_2 cipher_block plain_block 64ul;
-      (* Apply Salsa20 to the next blocks *)
-      salsa20_encrypt_loop state key counter nonce plaintext' ciphertext' (U32 (j +^ 1ul)) max
-    end
-
-
-#reset-options "--max_fuel 0 --initial_fuel 0 --initial_ifuel 0 --max_ifuel 0 --z3timeout 5"
-
-val salsa20_encrypt_body:
-  state:uint32_p{length state = 32} ->
-  ciphertext:uint8_p{disjoint state ciphertext} ->
-  key:uint8_p{length key = 32 /\ disjoint ciphertext key /\ disjoint key state} ->
-  counter:h64 ->
-  nonce:uint8_p{length nonce = 8 /\ disjoint ciphertext nonce /\ disjoint state nonce} ->
-  plaintext:uint8_p{disjoint ciphertext plaintext /\ disjoint state plaintext} ->
-  len:u32{length ciphertext >= FStar.UInt32.v len /\ length plaintext >= FStar.UInt32.v len /\ Hacl.UInt64.v counter + FStar.UInt32.v len / 64 < pow2 32} ->
-  Stack unit
-    (requires (fun h -> live h state /\ live h ciphertext /\ live h key /\ live h nonce /\ live h plaintext))
-    (ensures (fun h0 _ h1 -> live h1 ciphertext /\ live h1 state /\ modifies_2 ciphertext state h0 h1))
-let salsa20_encrypt_body state ciphertext key counter nonce plaintext len =
-  let max = U32 (len /^ 64ul) in
-  let rem = U32 (len %^ 64ul) in
-  (* Apply Salsa20 max times **)
-  salsa20_encrypt_loop state key counter nonce plaintext ciphertext 0ul max;
-  if rem =^ 0ul then ()
-  else
-    begin
-      let open FStar.Buffer in
-      let cipher_block = sub ciphertext (U32 (64ul *^ max)) rem in
-      let plain_block = sub plaintext (U32 (64ul *^ max)) rem in
-      let h = ST.get() in
-      salsa20_core cipher_block state key (H64 (counter +^ (uint32_to_sint64 max))) nonce rem;
-      xor_uint8_p_2 cipher_block plain_block rem
-    end
-
-
-val salsa20_encrypt:
-  ciphertext:uint8_p ->
-  key:uint8_p{length key = 32 /\ disjoint ciphertext key} ->
-  nonce:uint8_p{length nonce = 8 /\ disjoint ciphertext nonce /\ disjoint key nonce} ->
-  plaintext:uint8_p{disjoint ciphertext plaintext /\ disjoint key plaintext /\ disjoint nonce plaintext} ->
-  len:u32{length ciphertext >= FStar.UInt32.v len /\ length plaintext >= FStar.UInt32.v len /\ FStar.UInt32.v len / 64 < pow2 32} ->
-  Stack unit
-    (requires (fun h -> live h ciphertext /\ live h key /\ live h nonce /\ live h plaintext))
-    (ensures (fun h0 _ h1 -> live h1 ciphertext /\ modifies_1 ciphertext h0 h1))
-let salsa20_encrypt ciphertext key nonce plaintext len =
-  push_frame ();
-  let state = create (uint32_to_sint32 0ul) 32ul in
-  (* Compute number of iterations *)
-  let counter = uint64_to_sint64 0uL in
-  salsa20_encrypt_body state ciphertext key counter nonce plaintext len;
+  let zero = uint8_to_sint8 0uy in
+  let local_state = create zero 112ul in
+  let input = Buffer.sub local_state 0ul  16ul in
+  let block = Buffer.sub local_state 16ul 64ul in
+  let kcopy = Buffer.sub local_state 80ul 32ul in
+  (* let k0 = k.(0ul) in let k1 = k.(1ul) in let k2 = k.(2ul) in let k3 = k.(3ul) in *)
+  (* let k4 = k.(4ul) in let k5 = k.(5ul) in let k6 = k.(6ul) in let k7 = k.(7ul) in *)
+  (* let k8 = k.(8ul) in let k9 = k.(9ul) in let k10 = k.(10ul) in let k11 = k.(11ul) in *)
+  (* let k12 = k.(12ul) in let k13 = k.(13ul) in let k14 = k.(14ul) in let k15 = k.(15ul) in *)
+  (* let k16 = k.(16ul) in let k17 = k.(17ul) in let k18 = k.(18ul) in let k19 = k.(19ul) in *)
+  (* let k20 = k.(20ul) in let k21 = k.(21ul) in let k22 = k.(22ul) in let k23 = k.(23ul) in *)
+  (* let k24 = k.(24ul) in let k25 = k.(25ul) in let k26 = k.(26ul) in let k27 = k.(27ul) in *)
+  (* let k28 = k.(28ul) in let k29 = k.(29ul) in let k30 = k.(30ul) in let k31 = k.(31ul) in *)
+  (* let n0 = n.(0ul) in let n1 = n.(1ul) in let n2 = n.(2ul) in let n3 = n.(3ul) in *)
+  (* let n4 = n.(4ul) in let n5 = n.(5ul) in let n6 = n.(6ul) in let n7 = n.(7ul) in *)
+  (* kcopy.(0ul) <- k0;   kcopy.(1ul) <- k1; *)
+  (* kcopy.(2ul) <- k2;   kcopy.(3ul) <- k3; *)
+  (* kcopy.(4ul) <- k4;   kcopy.(5ul) <- k5; *)
+  (* kcopy.(6ul) <- k6;   kcopy.(7ul) <- k7; *)
+  (* kcopy.(8ul) <- k8;   kcopy.(9ul) <- k9; *)
+  (* kcopy.(10ul) <- k10; kcopy.(11ul) <- k11; *)
+  (* kcopy.(12ul) <- k12; kcopy.(13ul) <- k13; *)
+  (* kcopy.(14ul) <- k14; kcopy.(15ul) <- k15; *)
+  (* kcopy.(16ul) <- k16; kcopy.(17ul) <- k17; *)
+  (* kcopy.(18ul) <- k18; kcopy.(19ul) <- k19; *)
+  (* kcopy.(20ul) <- k20; kcopy.(21ul) <- k21; *)
+  (* kcopy.(22ul) <- k22; kcopy.(23ul) <- k23; *)
+  (* kcopy.(24ul) <- k24; kcopy.(25ul) <- k25; *)
+  (* kcopy.(26ul) <- k26; kcopy.(27ul) <- k27; *)
+  (* kcopy.(28ul) <- k28; kcopy.(29ul) <- k29; *)
+  (* kcopy.(30ul) <- k30; kcopy.(31ul) <- k31; *)
+  (* input.(0ul) <- n0;   input.(1ul) <- n1; *)
+  (* input.(2ul) <- n2;   input.(3ul) <- n3; *)
+  (* input.(4ul) <- n4;   input.(5ul) <- n5; *)
+  (* input.(6ul) <- n6;   input.(7ul) <- n7; *)
+  (* input.(8ul)  <- uint64_to_sint8 ic; *)
+  (* input.(9ul)  <- uint64_to_sint8 (FStar.UInt64 (ic >>^ 8ul)); *)
+  (* input.(10ul) <- uint64_to_sint8 (FStar.UInt64 (ic >>^ 16ul)); *)
+  (* input.(11ul) <- uint64_to_sint8 (FStar.UInt64 (ic >>^ 24ul)); *)
+  (* input.(12ul) <- uint64_to_sint8 (FStar.UInt64 (ic >>^ 32ul)); *)
+  (* input.(13ul) <- uint64_to_sint8 (FStar.UInt64 (ic >>^ 40ul)); *)
+  (* input.(14ul) <- uint64_to_sint8 (FStar.UInt64 (ic >>^ 48ul)); *)
+  (* input.(15ul) <- uint64_to_sint8 (FStar.UInt64 (ic >>^ 56ul)); *)
+  crypto_stream_salsa20_xor_ic__ n ic k local_state;
+  let h1 = ST.get() in
+  cut (modifies_0 h0 h1);
+  let _ = crypto_stream_salsa20_xor_ic_loop c m block input kcopy mlen in
+  let mlen' = mod_64 mlen in
+  let off = U32 (Int.Cast.uint64_to_uint32 mlen -^ mlen') in
+  let h2 = ST.get() in
+  cut (modifies_3 c input block h1 h2);
+  cut (live h2 block /\ live h2 c /\ disjoint block c);
+  if U32 (mlen' >=^ 0ul) then (
+    crypto_core_salsa20 block input kcopy;
+    xor_bytes (offset c off) (offset m off) block (mlen')
+  );
+  let h3 = ST.get() in
+  cut (modifies_2 c block h2 h3);
+  lemma_modifies_3_1 c input block h0 h1 h2 h3;
   pop_frame()
 
 
-val salsa20_encrypt_with_counter:
-  ciphertext:uint8_p ->
-  key:uint8_p{length key = 32 /\ disjoint ciphertext key} ->
-  nonce:uint8_p{length nonce = 8 /\ disjoint ciphertext nonce /\ disjoint key nonce} ->
-  plaintext:uint8_p{disjoint ciphertext plaintext /\ disjoint key plaintext /\ disjoint nonce plaintext} ->
-  len:u32{length ciphertext >= U32.v len /\ length plaintext >= U32.v len} ->
-  counter:h64{H64.v counter + U32.v len / 64 < pow2 32} ->
+#reset-options "--initial_fuel 0 --max_fuel 0 --z3timeout 10"
+
+val crypto_stream_salsa20_xor_ic:
+  c:uint8_p ->
+  m:uint8_p ->
+  mlen:FStar.UInt64.t{U64.v mlen <= length c /\ U64.v mlen <= length m} ->
+  n:uint8_p{length n = 8} ->
+  ic:FStar.UInt64.t ->
+  k:uint8_p{length k = 32} ->
   Stack unit
-    (requires (fun h -> live h ciphertext /\ live h key /\ live h nonce /\ live h plaintext))
-    (ensures (fun h0 _ h1 -> live h1 ciphertext /\ modifies_1 ciphertext h0 h1))
-let salsa20_encrypt_with_counter ciphertext key nonce plaintext len counter =
-  push_frame ();
-  let state = create (uint32_to_sint32 0ul) 32ul in
-  (* Compute number of iterations *)
-  salsa20_encrypt_body state ciphertext key counter nonce plaintext len;
+    (requires (fun h -> live h c /\ live h m /\ live h n /\ live h k))
+    (ensures  (fun h0 _ h1 -> live h1 c /\ modifies_1 c h0 h1))
+let crypto_stream_salsa20_xor_ic c m mlen n ic k =
+  if FStar.UInt64 (mlen =^ 0uL) then ()
+  else crypto_stream_salsa20_xor_ic_ c m mlen n ic k
+
+
+#reset-options "--initial_fuel 0 --max_fuel 0 --z3timeout 200"
+
+val crypto_stream_salsa20_loop:
+  c:uint8_p ->
+  clen:FStar.UInt64.t{U64.v clen <= length c} ->
+  n:uint8_p{length n = 8} ->
+  k:uint8_p{length k = 32} ->
+  input:uint8_p{length input = 16 /\ disjoint input c} ->
+  Stack FStar.UInt64.t
+    (requires (fun h -> live h c /\ live h n /\ live h k /\ live h input))
+    (ensures  (fun h0 _ h1 -> live h1 c /\ live h1 input /\ modifies_2 c input h0 h1))
+let rec crypto_stream_salsa20_loop c clen n k input =
+  if FStar.UInt64 (clen <^ 64uL) then clen
+  else (
+    crypto_core_salsa20 (Buffer.sub c 0ul 64ul) input k;
+    let i8 = input.(8ul) in
+    let i9 = input.(9ul) in
+    let i10 = input.(10ul) in
+    let i11 = input.(11ul) in
+    let i12 = input.(12ul) in
+    let i13 = input.(13ul) in
+    let i14 = input.(14ul) in
+    let i15 = input.(15ul) in
+    let u = Hacl.UInt64(
+      sint8_to_sint64 i8
+      +%^ (sint8_to_sint64 i9 <<^ 8ul)
+      +%^ (sint8_to_sint64 i10 <<^ 16ul)
+      +%^ (sint8_to_sint64 i11 <<^ 24ul)
+      +%^ (sint8_to_sint64 i12 <<^ 32ul)
+      +%^ (sint8_to_sint64 i13 <<^ 40ul)
+      +%^ (sint8_to_sint64 i14 <<^ 48ul)
+      +%^ (sint8_to_sint64 i15 <<^ 56ul)
+      +%^ (uint64_to_sint64 1uL)
+    ) in
+    input.(8ul)  <- sint64_to_sint8 u;
+    input.(9ul)  <- sint64_to_sint8 (Hacl.UInt64 (u >>^ 8ul));
+    input.(10ul) <- sint64_to_sint8 (Hacl.UInt64 (u >>^ 16ul));
+    input.(11ul) <- sint64_to_sint8 (Hacl.UInt64 (u >>^ 24ul));
+    input.(12ul) <- sint64_to_sint8 (Hacl.UInt64 (u >>^ 32ul));
+    input.(13ul) <- sint64_to_sint8 (Hacl.UInt64 (u >>^ 40ul));
+    input.(14ul) <- sint64_to_sint8 (Hacl.UInt64 (u >>^ 48ul));
+    input.(15ul) <- sint64_to_sint8 (Hacl.UInt64 (u >>^ 56ul));
+    let clen = FStar.UInt64 (clen -^ 64uL) in
+    let c = offset c 64ul in
+    crypto_stream_salsa20_loop c clen n k input
+  )
+
+
+#reset-options "--initial_fuel 0 --max_fuel 0 --z3timeout 200"
+
+
+let lemma_modifies_4 (c:uint8_p) (input:uint8_p) (block:uint8_p) h0 h1 h2 h3 : Lemma
+  (requires (live h0 c /\ ~(contains h0 input) /\ ~(contains h0 block)
+    /\ live h1 c /\ live h1 input /\ live h1 block
+    /\ live h2 c /\ live h2 input /\ live h2 block
+    /\ modifies_0 h0 h1 /\ modifies_2 c input h1 h2 /\ modifies_2 c block h2 h3))
+  (ensures (modifies_2_1 c h0 h3))
+  = lemma_reveal_modifies_0 h0 h1;
+    lemma_reveal_modifies_2 c input h1 h2;
+    lemma_reveal_modifies_2 c block h2 h3;
+    lemma_intro_modifies_2_1 c h0 h3
+
+
+#reset-options "--initial_fuel 0 --max_fuel 0 --z3timeout 100"
+
+val crypto_stream_salsa20_:
+  n:uint8_p{length n = 8} ->
+  k:uint8_p{length k = 32} ->
+  local_state:uint8_p{length local_state = 112} ->
+  Stack unit
+    (requires (fun h -> live h n /\ live h k /\ live h local_state))
+    (ensures  (fun h0 _ h1 -> live h1 local_state /\ modifies_1 local_state h0 h1))
+let crypto_stream_salsa20_ n k local_state =
+  let zero = Hacl.Cast.uint8_to_sint8 0uy in
+  let input = Buffer.sub local_state 0ul 16ul in
+  let block = Buffer.sub local_state 16ul 64ul in
+  let kcopy = Buffer.sub local_state 80ul 32ul in
+  let k0 = k.(0ul) in let k1 = k.(1ul) in let k2 = k.(2ul) in let k3 = k.(3ul) in
+  let k4 = k.(4ul) in let k5 = k.(5ul) in let k6 = k.(6ul) in let k7 = k.(7ul) in
+  let k8 = k.(8ul) in let k9 = k.(9ul) in let k10 = k.(10ul) in let k11 = k.(11ul) in
+  let k12 = k.(12ul) in let k13 = k.(13ul) in let k14 = k.(14ul) in let k15 = k.(15ul) in
+  let k16 = k.(16ul) in let k17 = k.(17ul) in let k18 = k.(18ul) in let k19 = k.(19ul) in
+  let k20 = k.(20ul) in let k21 = k.(21ul) in let k22 = k.(22ul) in let k23 = k.(23ul) in
+  let k24 = k.(24ul) in let k25 = k.(25ul) in let k26 = k.(26ul) in let k27 = k.(27ul) in
+  let k28 = k.(28ul) in let k29 = k.(29ul) in let k30 = k.(30ul) in let k31 = k.(31ul) in
+  let n0 = n.(0ul) in let n1 = n.(1ul) in let n2 = n.(2ul) in let n3 = n.(3ul) in
+  let n4 = n.(4ul) in let n5 = n.(5ul) in let n6 = n.(6ul) in let n7 = n.(7ul) in
+  kcopy.(0ul) <- k0;   kcopy.(1ul) <- k1;
+  kcopy.(2ul) <- k2;   kcopy.(3ul) <- k3;
+  kcopy.(4ul) <- k4;   kcopy.(5ul) <- k5;
+  kcopy.(6ul) <- k6;   kcopy.(7ul) <- k7;
+  kcopy.(8ul) <- k8;   kcopy.(9ul) <- k9;
+  kcopy.(10ul) <- k10; kcopy.(11ul) <- k11;
+  kcopy.(12ul) <- k12; kcopy.(13ul) <- k13;
+  kcopy.(14ul) <- k14; kcopy.(15ul) <- k15;
+  kcopy.(16ul) <- k16; kcopy.(17ul) <- k17;
+  kcopy.(18ul) <- k18; kcopy.(19ul) <- k19;
+  kcopy.(20ul) <- k20; kcopy.(21ul) <- k21;
+  kcopy.(22ul) <- k22; kcopy.(23ul) <- k23;
+  kcopy.(24ul) <- k24; kcopy.(25ul) <- k25;
+  kcopy.(26ul) <- k26; kcopy.(27ul) <- k27;
+  kcopy.(28ul) <- k28; kcopy.(29ul) <- k29;
+  kcopy.(30ul) <- k30; kcopy.(31ul) <- k31;
+  input.(0ul) <- n0;   input.(1ul) <- n1;
+  input.(2ul) <- n2;   input.(3ul) <- n3;
+  input.(4ul) <- n4;   input.(5ul) <- n5;
+  input.(6ul) <- n6;   input.(7ul) <- n7;
+  input.(8ul)  <- zero;
+  input.(9ul)  <- zero;
+  input.(10ul) <- zero;
+  input.(11ul) <- zero;
+  input.(12ul) <- zero;
+  input.(13ul) <- zero;
+  input.(14ul) <- zero;
+  input.(15ul) <- zero
+
+
+#reset-options "--initial_fuel 0 --max_fuel 0 --z3timeout 200"
+
+val crypto_stream_salsa20:
+  c:uint8_p ->
+  clen:FStar.UInt64.t{U64.v clen <= length c} ->
+  n:uint8_p{length n = 8} ->
+  k:uint8_p{length k = 32} ->
+  Stack unit
+    (requires (fun h -> live h c /\ live h n /\ live h k))
+    (ensures  (fun h0 _ h1 -> modifies_1 c h0 h1 /\ live h1 c))
+let crypto_stream_salsa20 c clen n k =
+  push_frame();
+  let hh = ST.get() in
+  if (FStar.UInt64 (clen =^ 0uL)) then (let h = ST.get() in lemma_intro_modifies_2_1 c h h)
+  else (
+    let clen' = mod_64 clen in
+    Math.Lemmas.modulo_lemma (U64.v clen) (pow2 32);
+    let off = U32 (Int.Cast.uint64_to_uint32 clen -^ clen') in
+    let h0 = ST.get() in
+    let zero = uint8_to_sint8 0uy in
+    let local_state = create zero 112ul in
+    let input = Buffer.sub local_state 0ul 16ul in
+    let block = Buffer.sub local_state 16ul 64ul in
+    let kcopy = Buffer.sub local_state 80ul 32ul in
+    (* let k0 = k.(0ul) in let k1 = k.(1ul) in let k2 = k.(2ul) in let k3 = k.(3ul) in *)
+    (* let k4 = k.(4ul) in let k5 = k.(5ul) in let k6 = k.(6ul) in let k7 = k.(7ul) in *)
+    (* let k8 = k.(8ul) in let k9 = k.(9ul) in let k10 = k.(10ul) in let k11 = k.(11ul) in *)
+    (* let k12 = k.(12ul) in let k13 = k.(13ul) in let k14 = k.(14ul) in let k15 = k.(15ul) in *)
+    (* let k16 = k.(16ul) in let k17 = k.(17ul) in let k18 = k.(18ul) in let k19 = k.(19ul) in *)
+    (* let k20 = k.(20ul) in let k21 = k.(21ul) in let k22 = k.(22ul) in let k23 = k.(23ul) in *)
+    (* let k24 = k.(24ul) in let k25 = k.(25ul) in let k26 = k.(26ul) in let k27 = k.(27ul) in *)
+    (* let k28 = k.(28ul) in let k29 = k.(29ul) in let k30 = k.(30ul) in let k31 = k.(31ul) in *)
+    (* let n0 = n.(0ul) in let n1 = n.(1ul) in let n2 = n.(2ul) in let n3 = n.(3ul) in *)
+    (* let n4 = n.(4ul) in let n5 = n.(5ul) in let n6 = n.(6ul) in let n7 = n.(7ul) in *)
+    (* kcopy.(0ul) <- k0;   kcopy.(1ul) <- k1; *)
+    (* kcopy.(2ul) <- k2;   kcopy.(3ul) <- k3; *)
+    (* kcopy.(4ul) <- k4;   kcopy.(5ul) <- k5; *)
+    (* kcopy.(6ul) <- k6;   kcopy.(7ul) <- k7; *)
+    (* kcopy.(8ul) <- k8;   kcopy.(9ul) <- k9; *)
+    (* kcopy.(10ul) <- k10; kcopy.(11ul) <- k11; *)
+    (* kcopy.(12ul) <- k12; kcopy.(13ul) <- k13; *)
+    (* kcopy.(14ul) <- k14; kcopy.(15ul) <- k15; *)
+    (* kcopy.(16ul) <- k16; kcopy.(17ul) <- k17; *)
+    (* kcopy.(18ul) <- k18; kcopy.(19ul) <- k19; *)
+    (* kcopy.(20ul) <- k20; kcopy.(21ul) <- k21; *)
+    (* kcopy.(22ul) <- k22; kcopy.(23ul) <- k23; *)
+    (* kcopy.(24ul) <- k24; kcopy.(25ul) <- k25; *)
+    (* kcopy.(26ul) <- k26; kcopy.(27ul) <- k27; *)
+    (* kcopy.(28ul) <- k28; kcopy.(29ul) <- k29; *)
+    (* kcopy.(30ul) <- k30; kcopy.(31ul) <- k31; *)
+    (* input.(0ul) <- n0;   input.(1ul) <- n1; *)
+    (* input.(2ul) <- n2;   input.(3ul) <- n3; *)
+    (* input.(4ul) <- n4;   input.(5ul) <- n5; *)
+    (* input.(6ul) <- n6;   input.(7ul) <- n7; *)
+    (* input.(8ul)  <- zero; *)
+    (* input.(9ul)  <- zero; *)
+    (* input.(10ul) <- zero; *)
+    (* input.(11ul) <- zero; *)
+    (* input.(12ul) <- zero; *)
+    (* input.(13ul) <- zero; *)
+    (* input.(14ul) <- zero; *)
+    (* input.(15ul) <- zero; *)
+    crypto_stream_salsa20_ n k local_state;
+    let h1 = ST.get() in
+    cut (modifies_0 h0 h1);
+    let _ = crypto_stream_salsa20_loop c clen n kcopy input in
+    let h2 = ST.get() in
+    cut (modifies_2 c input h1 h2);
+    if U32 (clen' >=^ 0ul) then (
+      crypto_core_salsa20 block input kcopy;
+      blit block 0ul (offset c off) 0ul (clen');
+      let h3 = ST.get() in
+      cut (modifies_2 c block h2 h3)
+    ) else (lemma_intro_modifies_2 c block h2 h2);
+    let h3 = ST.get() in
+    cut (modifies_2 c block h2 h3);
+    lemma_modifies_4 c input block h0 h1 h2 h3
+  );
+  let hhh = ST.get() in
+  cut (modifies_2_1 c hh hhh);
   pop_frame()
+
+
+val crypto_stream_salsa20_xor:
+  c:uint8_p ->
+  m:uint8_p ->
+  mlen:FStar.UInt64.t{U64.v mlen <= length c /\ U64.v mlen <= length m} ->
+  n:uint8_p{length n = 8} ->
+  k:uint8_p{length k = 32} ->
+  Stack unit
+    (requires (fun h -> live h c /\ live h m /\ live h n /\ live h k))
+    (ensures  (fun h0 _ h1 -> live h1 c /\ modifies_1 c h0 h1))
+let crypto_stream_salsa20_xor c m mlen n k =
+  crypto_stream_salsa20_xor_ic c m mlen n 0uL k
