crypto/symmetric/Hacl.Symmetric.XSalsa20.fst
@@ -1,125 +1,81 @@
 module Hacl.Symmetric.XSalsa20
 
-open FStar.Mul
-open FStar.Ghost
+
 open FStar.HyperStack
 open FStar.ST
-open FStar.UInt32
-open Hacl.UInt8
+open FStar.Buffer
 open Hacl.UInt32
 open Hacl.Cast
-open FStar.Buffer
 
-open Utils
-
-#reset-options "--max_fuel 0 --initial_fuel 0 --initial_ifuel 0 --max_ifuel 0"
-
-(* Module abbreviations *)
-module HH = FStar.HyperHeap
-module HS = FStar.HyperStack
-
-module U8  = FStar.UInt8
-module U32 = FStar.UInt32
-module H8  = Hacl.UInt8
-module H32  = Hacl.UInt32
-module H64  = Hacl.UInt64
-
+open Hacl.Symmetric.HSalsa20
 open Hacl.Symmetric.Salsa20
 
-val initialize_hsalsa_state:
-  state:uint32_p{length state >= 16} ->
-  key:uint8_p{length key = 32 /\ disjoint state key} ->
-  nonce:uint8_p{length nonce = 16 /\ disjoint state nonce} ->
+
+let h32 = Hacl.UInt32.t
+let u32 = FStar.UInt32.t
+let uint8_p = buffer Hacl.UInt8.t
+
+module U64 = FStar.UInt64
+module U32 = FStar.UInt32
+
+#reset-options "--initial_fuel 0 --max_fuel 0"
+
+private val lemma_max_uint32: n:nat -> Lemma
+  (requires (n = 32))
+  (ensures  (pow2 n = 4294967296))
+  [SMTPat (pow2 n)]
+let lemma_max_uint32 n = assert_norm(pow2 32 = 4294967296)
+private val lemma_max_uint64: n:nat -> Lemma
+  (requires (n = 64))
+  (ensures  (pow2 n = 18446744073709551616))
+  [SMTPat (pow2 n)]
+let lemma_max_uint64 n = assert_norm(pow2 64 = 18446744073709551616)
+
+
+#reset-options "--initial_fuel 0 --max_fuel 0 --z3timeout 20"
+
+val crypto_stream_xsalsa20:
+  c:uint8_p ->
+  clen:FStar.UInt64.t{U64.v clen <= length c} ->
+  n:uint8_p{length n = 24} ->
+  k:uint8_p{length k = 32} ->
   Stack unit
-    (requires (fun h -> live h state /\ live h key /\ live h nonce))
-    (ensures (fun h0 _ h1 -> live h1 state /\ modifies_1 state h0 h1))
-let initialize_hsalsa_state state key nonce =
-  (* Key part *)
-  let k0 = sub key 0ul  4ul in
-  let k1 = sub key 4ul  4ul in
-  let k2 = sub key 8ul  4ul in
-  let k3 = sub key 12ul 4ul in
-  let k4 = sub key 16ul 4ul in
-  let k5 = sub key 20ul 4ul in
-  let k6 = sub key 24ul 4ul in
-  let k7 = sub key 28ul 4ul in
-  let k0 =  (uint32_of_bytes k0) in
-  let k1 =  (uint32_of_bytes k1) in
-  let k2 =  (uint32_of_bytes k2) in
-  let k3 =  (uint32_of_bytes k3) in
-  let k4 =  (uint32_of_bytes k4) in
-  let k5 =  (uint32_of_bytes k5) in
-  let k6 =  (uint32_of_bytes k6) in
-  let k7 =  (uint32_of_bytes k7) in
-  (* Nonce part *)
-  let n0 = sub nonce 0ul  4ul in
-  let n1 = sub nonce 4ul  4ul in
-  let n2 = sub nonce 8ul  4ul in
-  let n3 = sub nonce 12ul 4ul in
-  let n0 =  (uint32_of_bytes n0) in
-  let n1 =  (uint32_of_bytes n1) in
-  let n2 =  (uint32_of_bytes n2) in
-  let n3 =  (uint32_of_bytes n3) in
-  let h0 = ST.get() in
-  (* Constant part *)
-  state.(0ul) <- (uint32_to_sint32 0x61707865ul);
-  state.(5ul) <- (uint32_to_sint32 0x3320646eul);
-  state.(10ul) <- (uint32_to_sint32 0x79622d32ul);
-  state.(15ul) <- (uint32_to_sint32 0x6b206574ul);
-  (* Update with key *)
-  state.(1ul) <-  (k0);
-  state.(2ul) <-  (k1);
-  state.(3ul) <-  (k2);
-  state.(4ul) <-  (k3);
-  state.(11ul) <- (k4);
-  state.(12ul) <- (k5);
-  state.(13ul) <- (k6);
-  state.(14ul) <- (k7);
-  (* Update with nonces *)
-  state.(6ul) <- (n0);
-  state.(7ul) <- (n1);
-  state.(8ul) <- (n2);
-  state.(9ul) <- (n3)
-
-
-val hsalsa_init:
-  subkey:uint8_p{length subkey = 32} ->
-  key:uint8_p{length key = 32 /\ disjoint key subkey} ->
-  nonce:uint8_p{length nonce = 16 /\ disjoint nonce subkey} ->
-  Stack unit
-    (requires (fun h -> live h subkey /\ live h key /\ live h nonce))
-    (ensures  (fun h0 _ h1 -> modifies_1 subkey h0 h1 /\ live h1 subkey))
-let hsalsa_init subkey key nonce_16 =
-  push_frame ();
-  let m = create (uint32_to_sint32 0ul) 16ul in
-  initialize_hsalsa_state m key nonce_16;
-  rounds m;
-  (* Subkey *)
-  bytes_of_uint32s (offset subkey  0ul) (offset m  0ul)  4ul;
-  bytes_of_uint32s (offset subkey  4ul) (offset m  5ul)  4ul;
-  bytes_of_uint32s (offset subkey  8ul) (offset m 10ul)  4ul;
-  bytes_of_uint32s (offset subkey 12ul) (offset m 15ul)  4ul;
-  bytes_of_uint32s (offset subkey 16ul) (offset m  6ul) 16ul;
-  pop_frame()
-
-
-val xsalsa20_encrypt:
-  ciphertext:uint8_p ->
-  key:uint8_p{length key = 32 /\ disjoint ciphertext key} ->
-  nonce:uint8_p{length nonce = 24 /\ disjoint ciphertext nonce /\ disjoint key nonce} ->
-  plaintext:uint8_p{disjoint ciphertext plaintext /\ disjoint key plaintext /\ disjoint nonce plaintext} ->
-  len:u32{length ciphertext >= FStar.UInt32.v len /\ length plaintext >= FStar.UInt32.v len /\ FStar.UInt32.v len / 64 < pow2 32} ->
-  Stack unit
-    (requires (fun h -> live h ciphertext /\ live h key /\ live h nonce /\ live h plaintext))
-    (ensures (fun h0 _ h1 -> live h1 ciphertext /\ modifies_1 ciphertext h0 h1))
-let xsalsa20_encrypt ciphertext key nonce plaintext len =
-  push_frame ();
+    (requires (fun h -> live h c /\ live h n /\ live h k))
+    (ensures  (fun h0 _ h1 -> modifies_1 c h0 h1 /\ live h1 c))
+let crypto_stream_xsalsa20 c clen n k =
+  push_frame();
   let subkey = create (uint8_to_sint8 0uy) 32ul in
-  let nonce_16 = sub nonce 0ul 16ul in
-  let nonce_8 = sub nonce 16ul 8ul in
-  (* HSalsa run *)
-  hsalsa_init subkey key nonce_16;
-  (* Salsa20 run *)
-  let counter = uint64_to_sint64 0uL in
-  salsa20_encrypt ciphertext subkey nonce_8 plaintext len;
+  crypto_core_hsalsa20 subkey (Buffer.sub n 0ul 16ul) k;
+  crypto_stream_salsa20 c clen (offset n 16ul) subkey;
   pop_frame()
+
+
+val crypto_stream_xsalsa20_xor_ic:
+  c:uint8_p ->
+  m:uint8_p ->
+  mlen:FStar.UInt64.t{U64.v mlen <= length c /\ U64.v mlen <= length m} ->
+  n:uint8_p{length n = 24} ->
+  ic:FStar.UInt64.t ->
+  k:uint8_p{length k = 32} ->
+  Stack unit
+    (requires (fun h -> live h c /\ live h m /\ live h n /\ live h k))
+    (ensures  (fun h0 _ h1 -> live h1 c /\ modifies_1 c h0 h1))
+let crypto_stream_xsalsa20_xor_ic c m mlen n ic k =
+  push_frame();
+  let subkey = create (uint8_to_sint8 0uy) 32ul in
+  crypto_core_hsalsa20 subkey (Buffer.sub n 0ul 16ul) k;
+  crypto_stream_salsa20_xor_ic c m mlen (offset n 16ul) ic subkey;
+  pop_frame()
+
+
+val crypto_stream_xsalsa20_xor:
+  c:uint8_p ->
+  m:uint8_p ->
+  mlen:FStar.UInt64.t{U64.v mlen <= length c /\ U64.v mlen <= length m} ->
+  n:uint8_p{length n = 24} ->
+  k:uint8_p{length k = 32} ->
+  Stack unit
+    (requires (fun h -> live h c /\ live h m /\ live h n /\ live h k))
+    (ensures  (fun h0 _ h1 -> live h1 c /\ modifies_1 c h0 h1))
+let crypto_stream_xsalsa20_xor c m mlen n k =
+  crypto_stream_xsalsa20_xor_ic c m mlen n 0uL k
